converted to Isar, simplifying recursion on class hierarchy

src/HOL/MicroJava/J/Eval.thy
@@ -7,20 +7,21 @@ Operational evaluation (big-step) semantics of the
 execution of Java expressions and statements
 *)
 
-Eval = State + WellType +
+theory Eval = State + WellType:
+
 consts
-  eval  :: "java_mb prog => (xstate \\<times> expr      \\<times> val      \\<times> xstate) set"
-  evals :: "java_mb prog => (xstate \\<times> expr list \\<times> val list \\<times> xstate) set"
-  exec  :: "java_mb prog => (xstate \\<times> stmt                 \\<times> xstate) set"
+  eval  :: "java_mb prog => (xstate \<times> expr      \<times> val      \<times> xstate) set"
+  evals :: "java_mb prog => (xstate \<times> expr list \<times> val list \<times> xstate) set"
+  exec  :: "java_mb prog => (xstate \<times> stmt                 \<times> xstate) set"
 
 syntax
   eval :: "[java_mb prog,xstate,expr,val,xstate] => bool "
-          ("_ \\<turnstile> _ -_\\<succ>_-> _" [51,82,60,82,82] 81)
+          ("_ \<turnstile> _ -_\<succ>_-> _" [51,82,60,82,82] 81)
   evals:: "[java_mb prog,xstate,expr list,
                         val list,xstate] => bool "
-          ("_ \\<turnstile> _ -_[\\<succ>]_-> _" [51,82,60,51,82] 81)
+          ("_ \<turnstile> _ -_[\<succ>]_-> _" [51,82,60,51,82] 81)
   exec :: "[java_mb prog,xstate,stmt,    xstate] => bool "
-          ("_ \\<turnstile> _ -_-> _" [51,82,60,82] 81)
+          ("_ \<turnstile> _ -_-> _" [51,82,60,82] 81)
 
 syntax (HTML)
   eval :: "[java_mb prog,xstate,expr,val,xstate] => bool "
@@ -33,112 +34,159 @@ syntax (HTML)
 
 
 translations
-  "G\\<turnstile>s -e \\<succ> v-> (x,s')" <= "(s, e, v, x, s') \\<in> eval  G"
-  "G\\<turnstile>s -e \\<succ> v->    s' " == "(s, e, v,    s') \\<in> eval  G"
-  "G\\<turnstile>s -e[\\<succ>]v-> (x,s')" <= "(s, e, v, x, s') \\<in> evals G"
-  "G\\<turnstile>s -e[\\<succ>]v->    s' " == "(s, e, v,    s') \\<in> evals G"
-  "G\\<turnstile>s -c    -> (x,s')" <= "(s, c, x, s') \\<in> exec G"
-  "G\\<turnstile>s -c    ->    s' " == "(s, c,    s') \\<in> exec G"
+  "G\<turnstile>s -e \<succ> v-> (x,s')" <= "(s, e, v, x, s') \<in> eval  G"
+  "G\<turnstile>s -e \<succ> v->    s' " == "(s, e, v,    s') \<in> eval  G"
+  "G\<turnstile>s -e[\<succ>]v-> (x,s')" <= "(s, e, v, x, s') \<in> evals G"
+  "G\<turnstile>s -e[\<succ>]v->    s' " == "(s, e, v,    s') \<in> evals G"
+  "G\<turnstile>s -c    -> (x,s')" <= "(s, c, x, s') \<in> exec G"
+  "G\<turnstile>s -c    ->    s' " == "(s, c,    s') \<in> exec G"
 
-inductive "eval G" "evals G" "exec G" intrs
+inductive "eval G" "evals G" "exec G" intros
 
 (* evaluation of expressions *)
 
   (* cf. 15.5 *)
-  XcptE "G\\<turnstile>(Some xc,s) -e\\<succ>arbitrary-> (Some xc,s)"
+  XcptE:"G\<turnstile>(Some xc,s) -e\<succ>arbitrary-> (Some xc,s)"
 
   (* cf. 15.8.1 *)
-  NewC  "[| h = heap s; (a,x) = new_Addr h;
-            h'= h(a\\<mapsto>(C,init_vars (fields (G,C)))) |] ==>
-         G\\<turnstile>Norm s -NewC C\\<succ>Addr a-> c_hupd h' (x,s)"
+  NewC: "[| h = heap s; (a,x) = new_Addr h;
+            h'= h(a\<mapsto>(C,init_vars (fields (G,C)))) |] ==>
+         G\<turnstile>Norm s -NewC C\<succ>Addr a-> c_hupd h' (x,s)"
 
   (* cf. 15.15 *)
-  Cast  "[| G\\<turnstile>Norm s0 -e\\<succ>v-> (x1,s1);
-            x2 = raise_if (\\<not> cast_ok G C (heap s1) v) ClassCast x1 |] ==>
-         G\\<turnstile>Norm s0 -Cast C e\\<succ>v-> (x2,s1)"
+  Cast: "[| G\<turnstile>Norm s0 -e\<succ>v-> (x1,s1);
+            x2 = raise_if (\<not> cast_ok G C (heap s1) v) ClassCast x1 |] ==>
+         G\<turnstile>Norm s0 -Cast C e\<succ>v-> (x2,s1)"
 
   (* cf. 15.7.1 *)
-  Lit   "G\\<turnstile>Norm s -Lit v\\<succ>v-> Norm s"
+  Lit:  "G\<turnstile>Norm s -Lit v\<succ>v-> Norm s"
 
-  BinOp "[| G\\<turnstile>Norm s -e1\\<succ>v1-> s1;
-            G\\<turnstile>s1     -e2\\<succ>v2-> s2;
+  BinOp:"[| G\<turnstile>Norm s -e1\<succ>v1-> s1;
+            G\<turnstile>s1     -e2\<succ>v2-> s2;
             v = (case bop of Eq  => Bool (v1 = v2)
                            | Add => Intg (the_Intg v1 + the_Intg v2)) |] ==>
-         G\\<turnstile>Norm s -BinOp bop e1 e2\\<succ>v-> s2"
+         G\<turnstile>Norm s -BinOp bop e1 e2\<succ>v-> s2"
 
   (* cf. 15.13.1, 15.2 *)
-  LAcc  "G\\<turnstile>Norm s -LAcc v\\<succ>the (locals s v)-> Norm s"
+  LAcc: "G\<turnstile>Norm s -LAcc v\<succ>the (locals s v)-> Norm s"
 
   (* cf. 15.25.1 *)
-  LAss  "[| G\\<turnstile>Norm s -e\\<succ>v-> (x,(h,l));
-            l' = (if x = None then l(va\\<mapsto>v) else l) |] ==>
-         G\\<turnstile>Norm s -va::=e\\<succ>v-> (x,(h,l'))"
+  LAss: "[| G\<turnstile>Norm s -e\<succ>v-> (x,(h,l));
+            l' = (if x = None then l(va\<mapsto>v) else l) |] ==>
+         G\<turnstile>Norm s -va::=e\<succ>v-> (x,(h,l'))"
 
 
   (* cf. 15.10.1, 15.2 *)
-  FAcc  "[| G\\<turnstile>Norm s0 -e\\<succ>a'-> (x1,s1); 
+  FAcc: "[| G\<turnstile>Norm s0 -e\<succ>a'-> (x1,s1); 
             v = the (snd (the (heap s1 (the_Addr a'))) (fn,T)) |] ==>
-         G\\<turnstile>Norm s0 -{T}e..fn\\<succ>v-> (np a' x1,s1)"
+         G\<turnstile>Norm s0 -{T}e..fn\<succ>v-> (np a' x1,s1)"
 
   (* cf. 15.25.1 *)
-  FAss  "[| G\\<turnstile>     Norm s0  -e1\\<succ>a'-> (x1,s1); a = the_Addr a';
-            G\\<turnstile>(np a' x1,s1) -e2\\<succ>v -> (x2,s2);
+  FAss: "[| G\<turnstile>     Norm s0  -e1\<succ>a'-> (x1,s1); a = the_Addr a';
+            G\<turnstile>(np a' x1,s1) -e2\<succ>v -> (x2,s2);
             h  = heap s2; (c,fs) = the (h a);
-            h' = h(a\\<mapsto>(c,(fs((fn,T)\\<mapsto>v)))) |] ==>
-         G\\<turnstile>Norm s0 -{T}e1..fn:=e2\\<succ>v-> c_hupd h' (x2,s2)"
+            h' = h(a\<mapsto>(c,(fs((fn,T)\<mapsto>v)))) |] ==>
+         G\<turnstile>Norm s0 -{T}e1..fn:=e2\<succ>v-> c_hupd h' (x2,s2)"
 
   (* cf. 15.11.4.1, 15.11.4.2, 15.11.4.4, 15.11.4.5, 14.15 *)
-  Call  "[| G\\<turnstile>Norm s0 -e\\<succ>a'-> s1; a = the_Addr a';
-            G\\<turnstile>s1 -ps[\\<succ>]pvs-> (x,(h,l)); dynT = fst (the (h a));
+  Call: "[| G\<turnstile>Norm s0 -e\<succ>a'-> s1; a = the_Addr a';
+            G\<turnstile>s1 -ps[\<succ>]pvs-> (x,(h,l)); dynT = fst (the (h a));
             (md,rT,pns,lvars,blk,res) = the (method (G,dynT) (mn,pTs));
-            G\\<turnstile>(np a' x,(h,(init_vars lvars)(pns[\\<mapsto>]pvs)(This\\<mapsto>a'))) -blk-> s3;
-            G\\<turnstile> s3 -res\\<succ>v -> (x4,s4) |] ==>
-         G\\<turnstile>Norm s0 -{C}e..mn({pTs}ps)\\<succ>v-> (x4,(heap s4,l))"
+            G\<turnstile>(np a' x,(h,(init_vars lvars)(pns[\<mapsto>]pvs)(This\<mapsto>a'))) -blk-> s3;
+            G\<turnstile> s3 -res\<succ>v -> (x4,s4) |] ==>
+         G\<turnstile>Norm s0 -{C}e..mn({pTs}ps)\<succ>v-> (x4,(heap s4,l))"
 
 
 (* evaluation of expression lists *)
 
   (* cf. 15.5 *)
-  XcptEs "G\\<turnstile>(Some xc,s) -e[\\<succ>]arbitrary-> (Some xc,s)"
+  XcptEs:"G\<turnstile>(Some xc,s) -e[\<succ>]arbitrary-> (Some xc,s)"
 
   (* cf. 15.11.??? *)
-  Nil   "G\\<turnstile>Norm s0 -[][\\<succ>][]-> Norm s0"
+  Nil:  "G\<turnstile>Norm s0 -[][\<succ>][]-> Norm s0"
 
   (* cf. 15.6.4 *)
-  Cons  "[| G\\<turnstile>Norm s0 -e  \\<succ> v -> s1;
-            G\\<turnstile>     s1 -es[\\<succ>]vs-> s2 |] ==>
-         G\\<turnstile>Norm s0 -e#es[\\<succ>]v#vs-> s2"
+  Cons: "[| G\<turnstile>Norm s0 -e  \<succ> v -> s1;
+            G\<turnstile>     s1 -es[\<succ>]vs-> s2 |] ==>
+         G\<turnstile>Norm s0 -e#es[\<succ>]v#vs-> s2"
 
 (* execution of statements *)
 
   (* cf. 14.1 *)
-  XcptS "G\\<turnstile>(Some xc,s) -c-> (Some xc,s)"
+  XcptS:"G\<turnstile>(Some xc,s) -c-> (Some xc,s)"
 
   (* cf. 14.5 *)
-  Skip  "G\\<turnstile>Norm s -Skip-> Norm s"
+  Skip: "G\<turnstile>Norm s -Skip-> Norm s"
 
   (* cf. 14.7 *)
-  Expr  "[| G\\<turnstile>Norm s0 -e\\<succ>v-> s1 |] ==>
-         G\\<turnstile>Norm s0 -Expr e-> s1"
+  Expr: "[| G\<turnstile>Norm s0 -e\<succ>v-> s1 |] ==>
+         G\<turnstile>Norm s0 -Expr e-> s1"
 
   (* cf. 14.2 *)
-  Comp  "[| G\\<turnstile>Norm s0 -c1-> s1;
-            G\\<turnstile>     s1 -c2-> s2|] ==>
-         G\\<turnstile>Norm s0 -c1;; c2-> s2"
+  Comp: "[| G\<turnstile>Norm s0 -c1-> s1;
+            G\<turnstile>     s1 -c2-> s2|] ==>
+         G\<turnstile>Norm s0 -c1;; c2-> s2"
 
   (* cf. 14.8.2 *)
-  Cond  "[| G\\<turnstile>Norm s0  -e\\<succ>v-> s1;
-            G\\<turnstile> s1 -(if the_Bool v then c1 else c2)-> s2|] ==>
-         G\\<turnstile>Norm s0 -If(e) c1 Else c2-> s2"
+  Cond: "[| G\<turnstile>Norm s0  -e\<succ>v-> s1;
+            G\<turnstile> s1 -(if the_Bool v then c1 else c2)-> s2|] ==>
+         G\<turnstile>Norm s0 -If(e) c1 Else c2-> s2"
 
   (* cf. 14.10, 14.10.1 *)
-  LoopF "[| G\\<turnstile>Norm s0 -e\\<succ>v-> s1; \\<not>the_Bool v |] ==>
-         G\\<turnstile>Norm s0 -While(e) c-> s1"
-  LoopT "[| G\\<turnstile>Norm s0 -e\\<succ>v-> s1;  the_Bool v;
-	    G\\<turnstile>s1 -c-> s2; G\\<turnstile>s2 -While(e) c-> s3 |] ==>
-         G\\<turnstile>Norm s0 -While(e) c-> s3"
+  LoopF:"[| G\<turnstile>Norm s0 -e\<succ>v-> s1; \<not>the_Bool v |] ==>
+         G\<turnstile>Norm s0 -While(e) c-> s1"
+  LoopT:"[| G\<turnstile>Norm s0 -e\<succ>v-> s1;  the_Bool v;
+	    G\<turnstile>s1 -c-> s2; G\<turnstile>s2 -While(e) c-> s3 |] ==>
+         G\<turnstile>Norm s0 -While(e) c-> s3"
 
-monos
-  if_def2
+lemmas eval_evals_exec_induct = eval_evals_exec.induct [complete_split]
+
+lemma NewCI: "[|new_Addr (heap s) = (a,x);  
+       s' = c_hupd (heap s(a\<mapsto>(C,init_vars (fields (G,C))))) (x,s)|] ==>  
+       G\<turnstile>Norm s -NewC C\<succ>Addr a-> s'"
+apply (simp (no_asm_simp))
+apply (rule eval_evals_exec.NewC)
+apply auto
+done
+
+lemma eval_evals_exec_no_xcpt: 
+ "!!s s'. (G\<turnstile>(x,s) -e \<succ>  v -> (x',s') --> x'=None --> x=None) \<and>  
+          (G\<turnstile>(x,s) -es[\<succ>]vs-> (x',s') --> x'=None --> x=None) \<and>  
+          (G\<turnstile>(x,s) -c       -> (x',s') --> x'=None --> x=None)"
+apply(simp (no_asm_simp) only: split_tupled_all)
+apply(rule eval_evals_exec_induct)
+apply(unfold c_hupd_def)
+apply(simp_all)
+done
+
+lemma eval_no_xcpt: "G\<turnstile>(x,s) -e\<succ>v-> (None,s') ==> x=None"
+apply (drule eval_evals_exec_no_xcpt [THEN conjunct1, THEN mp])
+apply (fast)
+done
+
+lemma evals_no_xcpt: "G\<turnstile>(x,s) -e[\<succ>]v-> (None,s') ==> x=None"
+apply (drule eval_evals_exec_no_xcpt [THEN conjunct2, THEN conjunct1, THEN mp])
+apply (fast)
+done
+
+lemma eval_evals_exec_xcpt: 
+"!!s s'. (G\<turnstile>(x,s) -e \<succ>  v -> (x',s') --> x=Some xc --> x'=Some xc \<and> s'=s) \<and>  
+         (G\<turnstile>(x,s) -es[\<succ>]vs-> (x',s') --> x=Some xc --> x'=Some xc \<and> s'=s) \<and>  
+         (G\<turnstile>(x,s) -c       -> (x',s') --> x=Some xc --> x'=Some xc \<and> s'=s)"
+apply (simp (no_asm_simp) only: split_tupled_all)
+apply (rule eval_evals_exec_induct)
+apply (unfold c_hupd_def)
+apply (simp_all)
+done
+
+lemma eval_xcpt: "G\<turnstile>(Some xc,s) -e\<succ>v-> (x',s') ==> x'=Some xc \<and>  s'=s"
+apply (drule eval_evals_exec_xcpt [THEN conjunct1, THEN mp])
+apply (fast)
+done
+
+lemma exec_xcpt: "G\<turnstile>(Some xc,s) -s0-> (x',s') ==> x'=Some xc \<and>  s'=s"
+apply (drule eval_evals_exec_xcpt [THEN conjunct2, THEN conjunct2, THEN mp])
+apply (fast)
+done
 
 end
