src/HOL/MicroJava/J/TypeRel.thy
@@ -6,18 +6,18 @@
 The relations between Java types
 *)
 
-TypeRel = Decl +
+theory TypeRel = Decl:
 
 consts
-  subcls1 :: "'c prog => (cname \\<times> cname) set"  (* subclass *)
-  widen   :: "'c prog => (ty    \\<times> ty   ) set"  (* widening *)
-  cast    :: "'c prog => (cname \\<times> cname) set"  (* casting *)
+  subcls1 :: "'c prog => (cname \<times> cname) set"  (* subclass *)
+  widen   :: "'c prog => (ty    \<times> ty   ) set"  (* widening *)
+  cast    :: "'c prog => (cname \<times> cname) set"  (* casting *)
 
 syntax
-  subcls1 :: "'c prog => [cname, cname] => bool" ("_ \\<turnstile> _ \\<prec>C1 _" [71,71,71] 70)
-  subcls  :: "'c prog => [cname, cname] => bool" ("_ \\<turnstile> _ \\<preceq>C _" [71,71,71] 70)
-  widen   :: "'c prog => [ty   , ty   ] => bool" ("_ \\<turnstile> _ \\<preceq> _" [71,71,71] 70)
-  cast    :: "'c prog => [cname, cname] => bool" ("_ \\<turnstile> _ \\<preceq>? _" [71,71,71] 70)
+  subcls1 :: "'c prog => [cname, cname] => bool" ("_ \<turnstile> _ \<prec>C1 _" [71,71,71] 70)
+  subcls  :: "'c prog => [cname, cname] => bool" ("_ \<turnstile> _ \<preceq>C _" [71,71,71] 70)
+  widen   :: "'c prog => [ty   , ty   ] => bool" ("_ \<turnstile> _ \<preceq> _" [71,71,71] 70)
+  cast    :: "'c prog => [cname, cname] => bool" ("_ \<turnstile> _ \<preceq>? _" [71,71,71] 70)
 
 syntax (HTML)
   subcls1 :: "'c prog => [cname, cname] => bool" ("_ |- _ <=C1 _" [71,71,71] 70)
@@ -26,58 +26,215 @@ syntax (HTML)
   cast    :: "'c prog => [cname, cname] => bool" ("_ |- _ <=? _" [71,71,71] 70)
 
 translations
-  "G\\<turnstile>C \\<prec>C1 D" == "(C,D) \\<in> subcls1 G"
-  "G\\<turnstile>C \\<preceq>C  D" == "(C,D) \\<in> (subcls1 G)^*"
-  "G\\<turnstile>S \\<preceq>   T" == "(S,T) \\<in> widen   G"
-  "G\\<turnstile>C \\<preceq>?  D" == "(C,D) \\<in> cast    G"
+  "G\<turnstile>C \<prec>C1 D" == "(C,D) \<in> subcls1 G"
+  "G\<turnstile>C \<preceq>C  D" == "(C,D) \<in> (subcls1 G)^*"
+  "G\<turnstile>S \<preceq>   T" == "(S,T) \<in> widen   G"
+  "G\<turnstile>C \<preceq>?  D" == "(C,D) \<in> cast    G"
 
 defs
 
   (* direct subclass, cf. 8.1.3 *)
- subcls1_def"subcls1 G \\<equiv> {(C,D). C\\<noteq>Object \\<and> (\\<exists>c. class G C=Some c \\<and> fst c=D)}"
+ subcls1_def: "subcls1 G \<equiv> {(C,D). C\<noteq>Object \<and> (\<exists>c. class G C=Some c \<and> fst c=D)}"
   
+lemma subcls1D: 
+  "G\<turnstile>C\<prec>C1D \<Longrightarrow> C \<noteq> Object \<and> (\<exists>fs ms. class G C = Some (D,fs,ms))"
+apply (unfold subcls1_def)
+apply auto
+done
+
+lemma subcls1I: "\<lbrakk>class G C = Some (D,rest); C \<noteq> Object\<rbrakk> \<Longrightarrow> G\<turnstile>C\<prec>C1D"
+apply (unfold subcls1_def)
+apply auto
+done
+
+lemma subcls1_def2: 
+"subcls1 G = (\<Sigma>C\<in>{C. is_class G C} . {D. C\<noteq>Object \<and> fst (the (class G C))=D})"
+apply (unfold subcls1_def is_class_def)
+apply auto
+done
+
+lemma finite_subcls1: "finite (subcls1 G)"
+apply(subst subcls1_def2)
+apply(rule finite_SigmaI [OF finite_is_class])
+apply(rule_tac B = "{fst (the (class G C))}" in finite_subset)
+apply  auto
+done
+
+lemma subcls_is_class: "(C,D) \<in> (subcls1 G)^+ ==> is_class G C"
+apply (unfold is_class_def)
+apply(erule trancl_trans_induct)
+apply (auto dest!: subcls1D)
+done
+
+lemma subcls_is_class2 [rule_format (no_asm)]: "G\<turnstile>C\<preceq>C D \<Longrightarrow> is_class G D \<longrightarrow> is_class G C"
+apply (unfold is_class_def)
+apply (erule rtrancl_induct)
+apply  (drule_tac [2] subcls1D)
+apply  auto
+done
+
+consts class_rec ::"'c prog \<times> cname \<Rightarrow> 
+        'a \<Rightarrow> (cname \<Rightarrow> fdecl list \<Rightarrow> 'c mdecl list \<Rightarrow> 'a \<Rightarrow> 'a) \<Rightarrow> 'a"
+recdef class_rec "same_fst (\<lambda>G. wf ((subcls1 G)^-1)) (\<lambda>G. (subcls1 G)^-1)"
+      "class_rec (G,C) = (\<lambda>t f. case class G C of None \<Rightarrow> arbitrary 
+                         | Some (D,fs,ms) \<Rightarrow> if wf ((subcls1 G)^-1) then 
+      f C fs ms (if C = Object then t else class_rec (G,D) t f) else arbitrary)"
+recdef_tc class_rec_tc: class_rec
+  apply (unfold same_fst_def)
+  apply (auto intro: subcls1I)
+  done
+
+lemma class_rec_lemma: "\<lbrakk> wf ((subcls1 G)^-1); class G C = Some (D,fs,ms)\<rbrakk> \<Longrightarrow>
+ class_rec (G,C) t f = f C fs ms (if C=Object then t else class_rec (G,D) t f)";
+  apply (rule class_rec_tc [THEN class_rec.simps 
+              [THEN trans [THEN fun_cong [THEN fun_cong]]]])
+  apply (rule ext, rule ext)
+  apply auto
+  done
+
 consts
 
-  method	:: "'c prog \\<times> cname => ( sig   \\<leadsto> cname \\<times> ty \\<times> 'c)"
-  field	:: "'c prog \\<times> cname => ( vname \\<leadsto> cname \\<times> ty)"
-  fields	:: "'c prog \\<times> cname => ((vname \\<times> cname) \\<times>  ty) list"
-
-constdefs       (* auxiliary relation for recursive definitions below *)
-
-  subcls1_rel	:: "(('c prog \\<times> cname) \\<times> ('c prog \\<times> cname)) set"
- "subcls1_rel == {((G,C),(G',C')). G = G' \\<and>  wf ((subcls1 G)^-1) \\<and>  G\\<turnstile>C'\\<prec>C1C}"
+  method :: "'c prog \<times> cname => ( sig   \<leadsto> cname \<times> ty \<times> 'c)" (* ###curry *)
+  field  :: "'c prog \<times> cname => ( vname \<leadsto> cname \<times> ty     )" (* ###curry *)
+  fields :: "'c prog \<times> cname => ((vname \<times> cname) \<times> ty) list" (* ###curry *)
 
 (* methods of a class, with inheritance, overriding and hiding, cf. 8.4.6 *)
-recdef method "subcls1_rel"
- "method (G,C) = (if wf((subcls1 G)^-1) then (case class G C of None =>arbitrary
-                   | Some (D,fs,ms) => (if C = Object then empty else 
-                                           if is_class G D then method (G,D) 
-                                                           else arbitrary) ++
-                                           map_of (map (\\<lambda>(s,  m ). 
-                                                        (s,(C,m))) ms))
-                  else arbitrary)"
+defs method_def: "method \<equiv> \<lambda>(G,C). class_rec (G,C) empty (\<lambda>C fs ms ts.
+                           ts ++ map_of (map (\<lambda>(s,m). (s,(C,m))) ms))"
+
+lemma method_rec_lemma: "[|class G C = Some (D,fs,ms); wf ((subcls1 G)^-1)|] ==>
+  method (G,C) = (if C = Object then empty else method (G,D)) ++  
+  map_of (map (\<lambda>(s,m). (s,(C,m))) ms)"
+apply (unfold method_def)
+apply (simp split del: split_if)
+apply (erule (1) class_rec_lemma [THEN trans]);
+apply auto
+done
+
 
 (* list of fields of a class, including inherited and hidden ones *)
-recdef fields  "subcls1_rel"
- "fields (G,C) = (if wf((subcls1 G)^-1) then (case class G C of None =>arbitrary
-                   | Some (D,fs,ms) => map (\\<lambda>(fn,ft). ((fn,C),ft)) fs@
-                                           (if C = Object then [] else 
-                                           if is_class G D then fields (G,D) 
-                                                           else arbitrary))
-                  else arbitrary)"
-defs
+defs fields_def: "fields \<equiv> \<lambda>(G,C). class_rec (G,C) []    (\<lambda>C fs ms ts.
+                           map (\<lambda>(fn,ft). ((fn,C),ft)) fs @ ts)"
 
-  field_def "field == map_of o (map (\\<lambda>((fn,fd),ft). (fn,(fd,ft)))) o fields"
+lemma fields_rec_lemma: "[|class G C = Some (D,fs,ms); wf ((subcls1 G)^-1)|] ==>
+ fields (G,C) = 
+  map (\<lambda>(fn,ft). ((fn,C),ft)) fs @ (if C = Object then [] else fields (G,D))"
+apply (unfold fields_def)
+apply (simp split del: split_if)
+apply (erule (1) class_rec_lemma [THEN trans]);
+apply auto
+done
 
-inductive "widen G" intrs (*widening, viz. method invocation conversion, cf. 5.3
+
+defs field_def: "field == map_of o (map (\<lambda>((fn,fd),ft). (fn,(fd,ft)))) o fields"
+
+lemma field_fields: 
+"field (G,C) fn = Some (fd, fT) \<Longrightarrow> map_of (fields (G,C)) (fn, fd) = Some fT"
+apply (unfold field_def)
+apply (rule table_of_remap_SomeD)
+apply simp
+done
+
+
+inductive "widen G" intros (*widening, viz. method invocation conversion,cf. 5.3
 			     i.e. sort of syntactic subtyping *)
-  refl	             "G\\<turnstile>      T \\<preceq> T" 	 (* identity conv., cf. 5.1.1 *)
-  subcls "G\\<turnstile>C\\<preceq>C D ==> G\\<turnstile>Class C \\<preceq> Class D"
-  null	             "G\\<turnstile>     NT \\<preceq> RefT R"
+  refl   [intro!, simp]:       "G\<turnstile>      T \<preceq> T" 	 (* identity conv., cf. 5.1.1 *)
+  subcls         : "G\<turnstile>C\<preceq>C D ==> G\<turnstile>Class C \<preceq> Class D"
+  null   [intro!]:             "G\<turnstile>     NT \<preceq> RefT R"
 
-inductive "cast G" intrs (* casting conversion, cf. 5.5 / 5.1.5 *)
-                         (* left out casts on primitve types    *)
-  widen	 "G\\<turnstile>C\\<preceq>C D ==> G\\<turnstile>C \\<preceq>? D"
-  subcls "G\\<turnstile>D\\<preceq>C C ==> G\\<turnstile>C \\<preceq>? D"
+inductive "cast G" intros (* casting conversion, cf. 5.5 / 5.1.5 *)
+                          (* left out casts on primitve types    *)
+  widen:  "G\<turnstile>C\<preceq>C D ==> G\<turnstile>C \<preceq>? D"
+  subcls: "G\<turnstile>D\<preceq>C C ==> G\<turnstile>C \<preceq>? D"
+
+lemma widen_PrimT_RefT [iff]: "(G\<turnstile>PrimT pT\<preceq>RefT rT) = False"
+apply (rule iffI)
+apply (erule widen.elims)
+apply auto
+done
+
+lemma widen_RefT: "G\<turnstile>RefT R\<preceq>T ==> \<exists>t. T=RefT t"
+apply (ind_cases "G\<turnstile>S\<preceq>T")
+apply auto
+done
+
+lemma widen_RefT2: "G\<turnstile>S\<preceq>RefT R ==> \<exists>t. S=RefT t"
+apply (ind_cases "G\<turnstile>S\<preceq>T")
+apply auto
+done
+
+lemma widen_Class: "G\<turnstile>Class C\<preceq>T ==> \<exists>D. T=Class D"
+apply (ind_cases "G\<turnstile>S\<preceq>T")
+apply auto
+done
+
+lemma widen_Class_NullT [iff]: "(G\<turnstile>Class C\<preceq>NT) = False"
+apply (rule iffI)
+apply (ind_cases "G\<turnstile>S\<preceq>T")
+apply auto
+done
+
+lemma widen_Class_Class [iff]: "(G\<turnstile>Class C\<preceq> Class D) = (G\<turnstile>C\<preceq>C D)"
+apply (rule iffI)
+apply (ind_cases "G\<turnstile>S\<preceq>T")
+apply (auto elim: widen.subcls)
+done
+
+lemma widen_trans [rule_format (no_asm)]: "G\<turnstile>S\<preceq>U ==> \<forall>T. G\<turnstile>U\<preceq>T --> G\<turnstile>S\<preceq>T"
+apply (erule widen.induct)
+apply   safe
+apply  (frule widen_Class)
+apply  (frule_tac [2] widen_RefT)
+apply  safe
+apply(erule (1) rtrancl_trans)
+done
+
+ML {* InductAttrib.print_global_rules(the_context()) *}
+ML {* set show_tags *}
+
+(*####theorem widen_trans: "\<lbrakk>G\<turnstile>S\<preceq>U; G\<turnstile>U\<preceq>T\<rbrakk> \<Longrightarrow> G\<turnstile>S\<preceq>T"
+proof -
+  assume "G\<turnstile>S\<preceq>U"
+  thus "\<And>T. G\<turnstile>U\<preceq>T \<Longrightarrow> G\<turnstile>S\<preceq>T" (*(is "PROP ?P S U")*)
+  proof (induct (*cases*) (open) (*?P S U*) rule: widen.induct [consumes 1])
+    case refl
+    fix T' assume "G\<turnstile>T\<preceq>T'" thus "G\<turnstile>T\<preceq>T'".
+      (* fix T' show "PROP ?P T T".*)
+  next
+    case subcls
+    fix T assume "G\<turnstile>Class D\<preceq>T"
+    then obtain E where "T = Class E" by (blast dest: widen_Class)
+    from prems show "G\<turnstile>Class C\<preceq>T" proof (auto elim: rtrancl_trans) qed
+  next
+    case null
+    fix RT assume "G\<turnstile>RefT R\<preceq>RT"
+    then obtain rt where "RT = RefT rt" by (blast dest: widen_RefT)
+    thus "G\<turnstile>NT\<preceq>RT" by auto
+  qed
+qed
+*)
+
+theorem widen_trans: "\<lbrakk>G\<turnstile>S\<preceq>U; G\<turnstile>U\<preceq>T\<rbrakk> \<Longrightarrow> G\<turnstile>S\<preceq>T"
+proof -
+  assume "G\<turnstile>S\<preceq>U"
+  thus "\<And>T. G\<turnstile>U\<preceq>T \<Longrightarrow> G\<turnstile>S\<preceq>T" (*(is "PROP ?P S U")*)
+  proof (induct (*cases*) (open) (*?P S U*)) (* rule: widen.induct *)
+    case refl
+    fix T' assume "G\<turnstile>T\<preceq>T'" thus "G\<turnstile>T\<preceq>T'".
+      (* fix T' show "PROP ?P T T".*)
+  next
+    case subcls
+    fix T assume "G\<turnstile>Class D\<preceq>T"
+    then obtain E where "T = Class E" by (blast dest: widen_Class)
+    from prems show "G\<turnstile>Class C\<preceq>T" proof (auto elim: rtrancl_trans) qed
+  next
+    case null
+    fix RT assume "G\<turnstile>RefT R\<preceq>RT"
+    then obtain rt where "RT = RefT rt" by (blast dest: widen_RefT)
+    thus "G\<turnstile>NT\<preceq>RT" by auto
+  qed
+qed
+
+
 
 end
