src/HOL/MicroJava/J/WellType.thy
@@ -15,41 +15,59 @@ simplifications:
 
 *)
 
-WellType = Term + WellForm +
+theory WellType = Term + WellForm:
 
 types	lenv (* local variables, including method parameters and This *)
-	= "vname \\<leadsto> ty"
+	= "vname \<leadsto> ty"
         'c env
-	= "'c prog \\<times> lenv"
+	= "'c prog \<times> lenv"
 
 syntax
   prg    :: "'c env => 'c prog"
-  localT :: "'c env => (vname \\<leadsto> ty)"
+  localT :: "'c env => (vname \<leadsto> ty)"
 
 translations	
   "prg"    => "fst"
   "localT" => "snd"
 
 consts
-  more_spec :: "'c prog => (ty \\<times> 'x) \\<times> ty list =>
-                (ty \\<times> 'x) \\<times> ty list => bool"
-  appl_methds :: "'c prog =>  cname => sig => ((ty \\<times> ty) \\<times> ty list) set"
-  max_spec :: "'c prog =>  cname => sig => ((ty \\<times> ty) \\<times> ty list) set"
+  more_spec :: "'c prog => (ty \<times> 'x) \<times> ty list =>
+                (ty \<times> 'x) \<times> ty list => bool"
+  appl_methds :: "'c prog =>  cname => sig => ((ty \<times> ty) \<times> ty list) set"
+  max_spec :: "'c prog =>  cname => sig => ((ty \<times> ty) \<times> ty list) set"
 
 defs
-  more_spec_def "more_spec G == \\<lambda>((d,h),pTs). \\<lambda>((d',h'),pTs'). G\\<turnstile>d\\<preceq>d' \\<and>
-		                            list_all2 (\\<lambda>T T'. G\\<turnstile>T\\<preceq>T') pTs pTs'"
+  more_spec_def: "more_spec G == \<lambda>((d,h),pTs). \<lambda>((d',h'),pTs'). G\<turnstile>d\<preceq>d' \<and>
+		                            list_all2 (\<lambda>T T'. G\<turnstile>T\<preceq>T') pTs pTs'"
   
   (* applicable methods, cf. 15.11.2.1 *)
-  appl_methds_def "appl_methds G C == \\<lambda>(mn, pTs).
+  appl_methds_def: "appl_methds G C == \<lambda>(mn, pTs).
 		                 {((Class md,rT),pTs') |md rT mb pTs'.
-		                  method (G,C)  (mn, pTs') = Some (md,rT,mb) \\<and>
-		                  list_all2 (\\<lambda>T T'. G\\<turnstile>T\\<preceq>T') pTs pTs'}"
+		                  method (G,C)  (mn, pTs') = Some (md,rT,mb) \<and>
+		                  list_all2 (\<lambda>T T'. G\<turnstile>T\<preceq>T') pTs pTs'}"
 
   (* maximally specific methods, cf. 15.11.2.2 *)
-  max_spec_def "max_spec G C sig == {m. m \\<in>appl_methds G C sig \\<and> 
-                                      (\\<forall>m'\\<in>appl_methds G C sig.
-                                        more_spec G m' m --> m' = m)}"
+  max_spec_def: "max_spec G C sig == {m. m \<in>appl_methds G C sig \<and> 
+                                       (\<forall>m'\<in>appl_methds G C sig.
+                                         more_spec G m' m --> m' = m)}"
+
+lemma max_spec2appl_meths: 
+  "x \<in> max_spec G C sig ==> x \<in> appl_methds G C sig"
+apply (unfold max_spec_def)
+apply (fast)
+done
+
+lemma appl_methsD: 
+"((md,rT),pTs')\<in>appl_methds G C (mn, pTs) ==>  
+  \<exists>D b. md = Class D \<and> method (G,C) (mn, pTs') = Some (D,rT,b)  
+  \<and> list_all2 (\<lambda>T T'. G\<turnstile>T\<preceq>T') pTs pTs'"
+apply (unfold appl_methds_def)
+apply (fast)
+done
+
+lemmas max_spec2mheads = insertI1 [THEN [2] equalityD2 [THEN subsetD], 
+                         THEN max_spec2appl_meths, THEN appl_methsD]
+
 
 consts
   typeof :: "(loc => ty option) => val => ty option"
@@ -61,19 +79,30 @@ primrec
 	"typeof dt (Intg i) = Some (PrimT Integer)"
 	"typeof dt (Addr a) = dt a"
 
+lemma is_type_typeof [rule_format (no_asm), simp]: "(\<forall>a. v \<noteq> Addr a) --> (\<exists>T. typeof t v = Some T \<and> is_type G T)"
+apply (rule val.induct)
+apply     auto
+done
+
+lemma typeof_empty_is_type [rule_format (no_asm)]: 
+  "typeof (\<lambda>a. None) v = Some T \<longrightarrow> is_type G T"
+apply (rule val.induct)
+apply     auto
+done
+
 types
-	java_mb = "vname list \\<times> (vname \\<times> ty) list \\<times> stmt \\<times> expr"
+	java_mb = "vname list \<times> (vname \<times> ty) list \<times> stmt \<times> expr"
 	(* method body with parameter names, local variables, block, result expression *)
 
 consts
-  ty_expr :: "java_mb env => (expr      \\<times> ty     ) set"
-  ty_exprs:: "java_mb env => (expr list \\<times> ty list) set"
+  ty_expr :: "java_mb env => (expr      \<times> ty     ) set"
+  ty_exprs:: "java_mb env => (expr list \<times> ty list) set"
   wt_stmt :: "java_mb env =>  stmt                 set"
 
 syntax
-  ty_expr :: "java_mb env => [expr     , ty     ] => bool" ("_ \\<turnstile> _ :: _"   [51,51,51]50)
-  ty_exprs:: "java_mb env => [expr list, ty list] => bool" ("_ \\<turnstile> _ [::] _" [51,51,51]50)
-  wt_stmt :: "java_mb env =>  stmt                => bool" ("_ \\<turnstile> _ \\<surd>"      [51,51   ]50)
+  ty_expr :: "java_mb env => [expr     , ty     ] => bool" ("_ \<turnstile> _ :: _"   [51,51,51]50)
+  ty_exprs:: "java_mb env => [expr list, ty list] => bool" ("_ \<turnstile> _ [::] _" [51,51,51]50)
+  wt_stmt :: "java_mb env =>  stmt                => bool" ("_ \<turnstile> _ \<surd>"      [51,51   ]50)
 
 syntax (HTML)
   ty_expr :: "java_mb env => [expr     , ty     ] => bool" ("_ |- _ :: _"   [51,51,51]50)
@@ -82,107 +111,123 @@ syntax (HTML)
 
 
 translations
-	"E\\<turnstile>e :: T" == "(e,T) \\<in> ty_expr  E"
-	"E\\<turnstile>e[::]T" == "(e,T) \\<in> ty_exprs E"
-	"E\\<turnstile>c \\<surd>"    == "c     \\<in> wt_stmt  E"
+	"E\<turnstile>e :: T" == "(e,T) \<in> ty_expr  E"
+	"E\<turnstile>e[::]T" == "(e,T) \<in> ty_exprs E"
+	"E\<turnstile>c \<surd>"    == "c     \<in> wt_stmt  E"
   
-inductive "ty_expr E" "ty_exprs E" "wt_stmt E" intrs
+inductive "ty_expr E" "ty_exprs E" "wt_stmt E" intros
 
 (* well-typed expressions *)
 
   (* cf. 15.8 *)
-  NewC	"[| is_class (prg E) C |] ==>
-         E\\<turnstile>NewC C::Class C"
+  NewC:	"[| is_class (prg E) C |] ==>
+         E\<turnstile>NewC C::Class C"
 
   (* cf. 15.15 *)
-  Cast  "[| E\\<turnstile>e::Class C; is_class (prg E) D;
-            prg E\\<turnstile>C\\<preceq>? D |] ==>
-         E\\<turnstile>Cast D e::Class D"
+  Cast:	"[| E\<turnstile>e::Class C; is_class (prg E) D;
+            prg E\<turnstile>C\<preceq>? D |] ==>
+         E\<turnstile>Cast D e::Class D"
 
   (* cf. 15.7.1 *)
-  Lit	  "[| typeof (\\<lambda>v. None) x = Some T |] ==>
-         E\\<turnstile>Lit x::T"
+  Lit:	  "[| typeof (\<lambda>v. None) x = Some T |] ==>
+         E\<turnstile>Lit x::T"
 
   
   (* cf. 15.13.1 *)
-  LAcc  "[| localT E v = Some T; is_type (prg E) T |] ==>
-         E\\<turnstile>LAcc v::T"
+  LAcc:	"[| localT E v = Some T; is_type (prg E) T |] ==>
+         E\<turnstile>LAcc v::T"
 
-  BinOp "[| E\\<turnstile>e1::T;
-            E\\<turnstile>e2::T;
+  BinOp:"[| E\<turnstile>e1::T;
+            E\<turnstile>e2::T;
             if bop = Eq then T' = PrimT Boolean
-                        else T' = T \\<and> T = PrimT Integer|] ==>
-         E\\<turnstile>BinOp bop e1 e2::T'"
+                        else T' = T \<and> T = PrimT Integer|] ==>
+         E\<turnstile>BinOp bop e1 e2::T'"
 
   (* cf. 15.25, 15.25.1 *)
-  LAss  "[| E\\<turnstile>LAcc v::T;
-	          E\\<turnstile>e::T';
-            prg E\\<turnstile>T'\\<preceq>T |] ==>
-         E\\<turnstile>v::=e::T'"
+  LAss: "[| E\<turnstile>LAcc v::T;
+	          E\<turnstile>e::T';
+            prg E\<turnstile>T'\<preceq>T |] ==>
+         E\<turnstile>v::=e::T'"
 
   (* cf. 15.10.1 *)
-  FAcc  "[| E\\<turnstile>a::Class C; 
+  FAcc: "[| E\<turnstile>a::Class C; 
             field (prg E,C) fn = Some (fd,fT) |] ==>
-         E\\<turnstile>{fd}a..fn::fT"
+         E\<turnstile>{fd}a..fn::fT"
 
   (* cf. 15.25, 15.25.1 *)
-  FAss  "[| E\\<turnstile>{fd}a..fn::T;
-            E\\<turnstile>v        ::T';
-            prg E\\<turnstile>T'\\<preceq>T |] ==>
-         E\\<turnstile>{fd}a..fn:=v::T'"
+  FAss: "[| E\<turnstile>{fd}a..fn::T;
+            E\<turnstile>v        ::T';
+            prg E\<turnstile>T'\<preceq>T |] ==>
+         E\<turnstile>{fd}a..fn:=v::T'"
 
 
   (* cf. 15.11.1, 15.11.2, 15.11.3 *)
-  Call  "[| E\\<turnstile>a::Class C;
-            E\\<turnstile>ps[::]pTs;
+  Call: "[| E\<turnstile>a::Class C;
+            E\<turnstile>ps[::]pTs;
             max_spec (prg E) C (mn, pTs) = {((md,rT),pTs')} |] ==>
-         E\\<turnstile>{C}a..mn({pTs'}ps)::rT"
+         E\<turnstile>{C}a..mn({pTs'}ps)::rT"
 
 (* well-typed expression lists *)
 
   (* cf. 15.11.??? *)
-  Nil  "E\\<turnstile>[][::][]"
+  Nil: "E\<turnstile>[][::][]"
 
   (* cf. 15.11.??? *)
-  Cons "[| E\\<turnstile>e::T;
-           E\\<turnstile>es[::]Ts |] ==>
-        E\\<turnstile>e#es[::]T#Ts"
+  Cons:"[| E\<turnstile>e::T;
+           E\<turnstile>es[::]Ts |] ==>
+        E\<turnstile>e#es[::]T#Ts"
 
 (* well-typed statements *)
 
-  Skip "E\\<turnstile>Skip\\<surd>"
+  Skip:"E\<turnstile>Skip\<surd>"
 
-  Expr "[| E\\<turnstile>e::T |] ==>
-        E\\<turnstile>Expr e\\<surd>"
+  Expr:"[| E\<turnstile>e::T |] ==>
+        E\<turnstile>Expr e\<surd>"
 
-  Comp "[| E\\<turnstile>s1\\<surd>; 
-           E\\<turnstile>s2\\<surd> |] ==>
-        E\\<turnstile>s1;; s2\\<surd>"
+  Comp:"[| E\<turnstile>s1\<surd>; 
+           E\<turnstile>s2\<surd> |] ==>
+        E\<turnstile>s1;; s2\<surd>"
 
   (* cf. 14.8 *)
-  Cond "[| E\\<turnstile>e::PrimT Boolean;
-           E\\<turnstile>s1\\<surd>;
-           E\\<turnstile>s2\\<surd> |] ==>
-         E\\<turnstile>If(e) s1 Else s2\\<surd>"
+  Cond:"[| E\<turnstile>e::PrimT Boolean;
+           E\<turnstile>s1\<surd>;
+           E\<turnstile>s2\<surd> |] ==>
+         E\<turnstile>If(e) s1 Else s2\<surd>"
 
   (* cf. 14.10 *)
-  Loop "[| E\\<turnstile>e::PrimT Boolean;
-           E\\<turnstile>s\\<surd> |] ==>
-        E\\<turnstile>While(e) s\\<surd>"
+  Loop:"[| E\<turnstile>e::PrimT Boolean;
+           E\<turnstile>s\<surd> |] ==>
+        E\<turnstile>While(e) s\<surd>"
 
 constdefs
 
- wf_java_mdecl :: java_mb prog => cname => java_mb mdecl => bool
-"wf_java_mdecl G C == \\<lambda>((mn,pTs),rT,(pns,lvars,blk,res)).
-	length pTs = length pns \\<and>
-	nodups pns \\<and>
-	unique lvars \\<and>
-	(\\<forall>pn\\<in>set pns. map_of lvars pn = None) \\<and>
-	(\\<forall>(vn,T)\\<in>set lvars. is_type G T) &
-	(let E = (G,map_of lvars(pns[\\<mapsto>]pTs)(This\\<mapsto>Class C)) in
-	 E\\<turnstile>blk\\<surd> \\<and> (\\<exists>T. E\\<turnstile>res::T \\<and> G\\<turnstile>T\\<preceq>rT))"
+ wf_java_mdecl :: "java_mb prog => cname => java_mb mdecl => bool"
+"wf_java_mdecl G C == \<lambda>((mn,pTs),rT,(pns,lvars,blk,res)).
+	length pTs = length pns \<and>
+	nodups pns \<and>
+	unique lvars \<and>
+	(\<forall>pn\<in>set pns. map_of lvars pn = None) \<and>
+	(\<forall>(vn,T)\<in>set lvars. is_type G T) &
+	(let E = (G,map_of lvars(pns[\<mapsto>]pTs)(This\<mapsto>Class C)) in
+	 E\<turnstile>blk\<surd> \<and> (\<exists>T. E\<turnstile>res::T \<and> G\<turnstile>T\<preceq>rT))"
 
- wf_java_prog :: java_mb prog => bool
+ wf_java_prog :: "java_mb prog => bool"
 "wf_java_prog G == wf_prog wf_java_mdecl G"
+
+
+lemma wt_is_type: "wf_prog wf_mb G \<Longrightarrow> ((G,L)\<turnstile>e::T \<longrightarrow> is_type G T) \<and>  
+       ((G,L)\<turnstile>es[::]Ts \<longrightarrow> Ball (set Ts) (is_type G)) \<and> ((G,L)\<turnstile>c \<surd> \<longrightarrow> True)"
+apply (rule ty_expr_ty_exprs_wt_stmt.induct)
+apply auto
+apply (   erule typeof_empty_is_type)
+apply (  simp split add: split_if_asm)
+apply ( drule field_fields)
+apply ( drule (1) fields_is_type)
+apply (  simp (no_asm_simp))
+apply  (assumption)
+apply (auto dest!: max_spec2mheads method_wf_mdecl is_type_rTI simp add: wf_mdecl_def)
+done
+
+lemmas ty_expr_is_type = wt_is_type [THEN conjunct1,THEN mp, COMP swap_prems_rl]
 
 end
