src/HOL/MicroJava/J/Conform.thy
@@ -6,30 +6,30 @@
 Conformity relations for type safety of Java
 *)
 
-Conform = State + WellType +
+theory Conform = State + WellType:
 
-types	'c env_ = "'c prog \\<times> (vname \\<leadsto> ty)" (* same as env of WellType.thy *)
+types	'c env_ = "'c prog \<times> (vname \<leadsto> ty)" (* same as env of WellType.thy *)
 
 constdefs
 
-  hext :: "aheap => aheap => bool" ("_ \\<le>| _" [51,51] 50)
- "h\\<le>|h' == \\<forall>a C fs. h a = Some(C,fs) --> (\\<exists>fs'. h' a = Some(C,fs'))"
+  hext :: "aheap => aheap => bool" ("_ \<le>| _" [51,51] 50)
+ "h\<le>|h' == \<forall>a C fs. h a = Some(C,fs) --> (\<exists>fs'. h' a = Some(C,fs'))"
 
-  conf :: "'c prog => aheap => val => ty => bool"	("_,_ \\<turnstile> _ ::\\<preceq> _" [51,51,51,51] 50)
- "G,h\\<turnstile>v::\\<preceq>T == \\<exists>T'. typeof (option_map obj_ty o h) v = Some T' \\<and> G\\<turnstile>T'\\<preceq>T"
+  conf :: "'c prog => aheap => val => ty => bool"	("_,_ \<turnstile> _ ::\<preceq> _" [51,51,51,51] 50)
+ "G,h\<turnstile>v::\<preceq>T == \<exists>T'. typeof (option_map obj_ty o h) v = Some T' \<and> G\<turnstile>T'\<preceq>T"
 
-  lconf :: "'c prog => aheap => ('a \\<leadsto> val) => ('a \\<leadsto> ty) => bool"
-                                                ("_,_ \\<turnstile> _ [::\\<preceq>] _" [51,51,51,51] 50)
- "G,h\\<turnstile>vs[::\\<preceq>]Ts == \\<forall>n T. Ts n = Some T --> (\\<exists>v. vs n = Some v \\<and> G,h\\<turnstile>v::\\<preceq>T)"
+  lconf :: "'c prog => aheap => ('a \<leadsto> val) => ('a \<leadsto> ty) => bool"
+                                                ("_,_ \<turnstile> _ [::\<preceq>] _" [51,51,51,51] 50)
+ "G,h\<turnstile>vs[::\<preceq>]Ts == \<forall>n T. Ts n = Some T --> (\<exists>v. vs n = Some v \<and> G,h\<turnstile>v::\<preceq>T)"
 
-  oconf :: "'c prog => aheap => obj => bool" ("_,_ \\<turnstile> _ \\<surd>" [51,51,51] 50)
- "G,h\\<turnstile>obj\\<surd> == G,h\\<turnstile>snd obj[::\\<preceq>]map_of (fields (G,fst obj))"
+  oconf :: "'c prog => aheap => obj => bool" ("_,_ \<turnstile> _ \<surd>" [51,51,51] 50)
+ "G,h\<turnstile>obj\<surd> == G,h\<turnstile>snd obj[::\<preceq>]map_of (fields (G,fst obj))"
 
-  hconf :: "'c prog => aheap => bool" ("_ \\<turnstile>h _ \\<surd>" [51,51] 50)
- "G\\<turnstile>h h\\<surd>    == \\<forall>a obj. h a = Some obj --> G,h\\<turnstile>obj\\<surd>"
+  hconf :: "'c prog => aheap => bool" ("_ \<turnstile>h _ \<surd>" [51,51] 50)
+ "G\<turnstile>h h\<surd>    == \<forall>a obj. h a = Some obj --> G,h\<turnstile>obj\<surd>"
 
-  conforms :: "state => java_mb env_ => bool"	("_ ::\\<preceq> _" [51,51] 50)
- "s::\\<preceq>E == prg E\\<turnstile>h heap s\\<surd> \\<and> prg E,heap s\\<turnstile>locals s[::\\<preceq>]localT E"
+  conforms :: "state => java_mb env_ => bool"	("_ ::\<preceq> _" [51,51] 50)
+ "s::\<preceq>E == prg E\<turnstile>h heap s\<surd> \<and> prg E,heap s\<turnstile>locals s[::\<preceq>]localT E"
 
 
 syntax (HTML)
@@ -39,7 +39,7 @@ syntax (HTML)
   conf     :: "'c prog => aheap => val => ty => bool"
               ("_,_ |- _ ::<= _"  [51,51,51,51] 50)
 
-  lconf    :: "'c prog => aheap => ('a \\<leadsto> val) => ('a \\<leadsto> ty) => bool"
+  lconf    :: "'c prog => aheap => ('a \<leadsto> val) => ('a \<leadsto> ty) => bool"
               ("_,_ |- _ [::<=] _" [51,51,51,51] 50)
 
   oconf    :: "'c prog => aheap => obj => bool"
@@ -50,5 +50,258 @@ syntax (HTML)
 
   conforms :: "state => java_mb env_ => bool"
               ("_ ::<= _" [51,51] 50)
+
+
+section "hext"
+
+lemma hextI: 
+" \<forall>a C fs . h  a = Some (C,fs) -->   
+      (\<exists>fs'. h' a = Some (C,fs')) ==> h\<le>|h'"
+apply (unfold hext_def)
+apply auto
+done
+
+lemma hext_objD: "[|h\<le>|h'; h a = Some (C,fs) |] ==> \<exists>fs'. h' a = Some (C,fs')"
+apply (unfold hext_def)
+apply (force)
+done
+
+lemma hext_refl [simp]: "h\<le>|h"
+apply (rule hextI)
+apply (fast)
+done
+
+lemma hext_new [simp]: "h a = None ==> h\<le>|h(a\<mapsto>x)"
+apply (rule hextI)
+apply auto
+done
+
+lemma hext_trans: "[|h\<le>|h'; h'\<le>|h''|] ==> h\<le>|h''"
+apply (rule hextI)
+apply (fast dest: hext_objD)
+done
+
+lemma hext_upd_obj: "h a = Some (C,fs) ==> h\<le>|h(a\<mapsto>(C,fs'))"
+apply (rule hextI)
+apply auto
+done
+
+
+section "conf"
+
+lemma conf_Null [simp]: "G,h\<turnstile>Null::\<preceq>T = G\<turnstile>RefT NullT\<preceq>T"
+apply (unfold conf_def)
+apply (simp (no_asm))
+done
+
+lemma conf_litval [rule_format (no_asm), simp]: 
+  "typeof (\<lambda>v. None) v = Some T --> G,h\<turnstile>v::\<preceq>T"
+apply (unfold conf_def)
+apply (rule val.induct)
+apply auto
+done
+
+lemma conf_AddrI: "[|h a = Some obj; G\<turnstile>obj_ty obj\<preceq>T|] ==> G,h\<turnstile>Addr a::\<preceq>T"
+apply (unfold conf_def)
+apply (simp)
+done
+
+lemma conf_obj_AddrI: "[|h a = Some (C,fs); G\<turnstile>C\<preceq>C D|] ==> G,h\<turnstile>Addr a::\<preceq> Class D"
+apply (unfold conf_def)
+apply (simp)
+done
+
+lemma defval_conf [rule_format (no_asm)]: "is_type G T --> G,h\<turnstile>default_val T::\<preceq>T"
+apply (unfold conf_def)
+apply (rule_tac "y" = "T" in ty.exhaust)
+apply  (erule ssubst)
+apply  (rule_tac "y" = "prim_ty" in prim_ty.exhaust)
+apply    (auto simp add: widen.null)
+done
+
+lemma conf_upd_obj: 
+"h a = Some (C,fs) ==> (G,h(a\<mapsto>(C,fs'))\<turnstile>x::\<preceq>T) = (G,h\<turnstile>x::\<preceq>T)"
+apply (unfold conf_def)
+apply (rule val.induct)
+apply auto
+done
+
+lemma conf_widen [rule_format (no_asm)]: "wf_prog wf_mb G ==> G,h\<turnstile>x::\<preceq>T --> G\<turnstile>T\<preceq>T' --> G,h\<turnstile>x::\<preceq>T'"
+apply (unfold conf_def)
+apply (rule val.induct)
+apply (auto intro: widen_trans)
+done
+
+lemma conf_hext [rule_format (no_asm)]: "h\<le>|h' ==> G,h\<turnstile>v::\<preceq>T --> G,h'\<turnstile>v::\<preceq>T"
+apply (unfold conf_def)
+apply (rule val.induct)
+apply (auto dest: hext_objD)
+done
+
+lemma new_locD: "[|h a = None; G,h\<turnstile>Addr t::\<preceq>T|] ==> t\<noteq>a"
+apply (unfold conf_def)
+apply auto
+done
+
+lemma conf_RefTD [rule_format (no_asm)]: 
+ "G,h\<turnstile>a'::\<preceq>RefT T --> a' = Null |   
+  (\<exists>a obj T'. a' = Addr a \<and>  h a = Some obj \<and>  obj_ty obj = T' \<and>  G\<turnstile>T'\<preceq>RefT T)"
+apply (unfold conf_def)
+apply(induct_tac "a'")
+apply(auto)
+done
+
+lemma conf_NullTD: "G,h\<turnstile>a'::\<preceq>RefT NullT ==> a' = Null"
+apply (drule conf_RefTD)
+apply auto
+done
+
+lemma non_npD: "[|a' \<noteq> Null; G,h\<turnstile>a'::\<preceq>RefT t|] ==>  
+  \<exists>a C fs. a' = Addr a \<and>  h a = Some (C,fs) \<and>  G\<turnstile>Class C\<preceq>RefT t"
+apply (drule conf_RefTD)
+apply auto
+done
+
+lemma non_np_objD: "!!G. [|a' \<noteq> Null; G,h\<turnstile>a'::\<preceq> Class C; C \<noteq> Object|] ==>  
+  (\<exists>a C' fs. a' = Addr a \<and>  h a = Some (C',fs) \<and>  G\<turnstile>C'\<preceq>C C)"
+apply (fast dest: non_npD)
+done
+
+lemma non_np_objD' [rule_format (no_asm)]: "a' \<noteq> Null ==> wf_prog wf_mb G ==> G,h\<turnstile>a'::\<preceq>RefT t --> 
+  (\<forall>C. t = ClassT C --> C \<noteq> Object) -->  
+  (\<exists>a C fs. a' = Addr a \<and>  h a = Some (C,fs) \<and>  G\<turnstile>Class C\<preceq>RefT t)"
+apply(rule_tac "y" = "t" in ref_ty.exhaust)
+ apply (fast dest: conf_NullTD)
+apply (fast dest: non_np_objD)
+done
+
+lemma conf_list_gext_widen [rule_format (no_asm)]: "wf_prog wf_mb G ==> \<forall>Ts Ts'. list_all2 (conf G h) vs Ts --> list_all2 (\<lambda>T T'. G\<turnstile>T\<preceq>T') Ts Ts' -->  list_all2 (conf G h) vs Ts'"
+apply(induct_tac "vs")
+ apply(clarsimp)
+apply(clarsimp)
+apply(frule list_all2_lengthD [THEN sym])
+apply(simp (no_asm_use) add: length_Suc_conv)
+apply(safe)
+apply(frule list_all2_lengthD [THEN sym])
+apply(simp (no_asm_use) add: length_Suc_conv)
+apply(clarify)
+apply(fast elim: conf_widen)
+done
+
+
+section "lconf"
+
+lemma lconfD: "[| G,h\<turnstile>vs[::\<preceq>]Ts; Ts n = Some T |] ==> G,h\<turnstile>(the (vs n))::\<preceq>T"
+apply (unfold lconf_def)
+apply (force)
+done
+
+lemma lconf_hext [elim]: "[| G,h\<turnstile>l[::\<preceq>]L; h\<le>|h' |] ==> G,h'\<turnstile>l[::\<preceq>]L"
+apply (unfold lconf_def)
+apply  (fast elim: conf_hext)
+done
+
+lemma lconf_upd: "!!X. [| G,h\<turnstile>l[::\<preceq>]lT;  
+  G,h\<turnstile>v::\<preceq>T; lT va = Some T |] ==> G,h\<turnstile>l(va\<mapsto>v)[::\<preceq>]lT"
+apply (unfold lconf_def)
+apply auto
+done
+
+lemma lconf_init_vars_lemma [rule_format (no_asm)]: "\<forall>x. P x --> R (dv x) x ==> (\<forall>x. map_of fs f = Some x --> P x) -->  
+  (\<forall>T. map_of fs f = Some T -->  
+  (\<exists>v. map_of (map (\<lambda>(f,ft). (f, dv ft)) fs) f = Some v \<and>  R v T))"
+apply( induct_tac "fs")
+apply auto
+done
+
+lemma lconf_init_vars [intro!]: 
+"\<forall>n. \<forall>T. map_of fs n = Some T --> is_type G T ==> G,h\<turnstile>init_vars fs[::\<preceq>]map_of fs"
+apply (unfold lconf_def init_vars_def)
+apply auto
+apply( rule lconf_init_vars_lemma)
+apply(   erule_tac [3] asm_rl)
+apply(  intro strip)
+apply(  erule defval_conf)
+apply auto
+done
+
+lemma lconf_ext: "[|G,s\<turnstile>l[::\<preceq>]L; G,s\<turnstile>v::\<preceq>T|] ==> G,s\<turnstile>l(vn\<mapsto>v)[::\<preceq>]L(vn\<mapsto>T)"
+apply (unfold lconf_def)
+apply auto
+done
+
+lemma lconf_ext_list [rule_format (no_asm)]: "G,h\<turnstile>l[::\<preceq>]L ==> \<forall>vs Ts. nodups vns --> length Ts = length vns --> list_all2 (\<lambda>v T. G,h\<turnstile>v::\<preceq>T) vs Ts --> G,h\<turnstile>l(vns[\<mapsto>]vs)[::\<preceq>]L(vns[\<mapsto>]Ts)"
+apply (unfold lconf_def)
+apply( induct_tac "vns")
+apply(  clarsimp)
+apply( clarsimp)
+apply( frule list_all2_lengthD)
+apply( auto simp add: length_Suc_conv)
+done
+
+
+section "oconf"
+
+lemma oconf_hext: "G,h\<turnstile>obj\<surd> ==> h\<le>|h' ==> G,h'\<turnstile>obj\<surd>"
+apply (unfold oconf_def)
+apply (fast)
+done
+
+lemma oconf_obj: "G,h\<turnstile>(C,fs)\<surd> =  
+  (\<forall>T f. map_of(fields (G,C)) f = Some T --> (\<exists>v. fs f = Some v \<and>  G,h\<turnstile>v::\<preceq>T))"
+apply (unfold oconf_def lconf_def)
+apply auto
+done
+
+lemmas oconf_objD = oconf_obj [THEN iffD1, THEN spec, THEN spec, THEN mp]
+
+
+section "hconf"
+
+lemma hconfD: "[|G\<turnstile>h h\<surd>; h a = Some obj|] ==> G,h\<turnstile>obj\<surd>"
+apply (unfold hconf_def)
+apply (fast)
+done
+
+lemma hconfI: "\<forall>a obj. h a=Some obj --> G,h\<turnstile>obj\<surd> ==> G\<turnstile>h h\<surd>"
+apply (unfold hconf_def)
+apply (fast)
+done
+
+
+section "conforms"
+
+lemma conforms_heapD: "(h, l)::\<preceq>(G, lT) ==> G\<turnstile>h h\<surd>"
+apply (unfold conforms_def)
+apply (simp)
+done
+
+lemma conforms_localD: "(h, l)::\<preceq>(G, lT) ==> G,h\<turnstile>l[::\<preceq>]lT"
+apply (unfold conforms_def)
+apply (simp)
+done
+
+lemma conformsI: "[|G\<turnstile>h h\<surd>; G,h\<turnstile>l[::\<preceq>]lT|] ==> (h, l)::\<preceq>(G, lT)"
+apply (unfold conforms_def)
+apply auto
+done
+
+lemma conforms_hext: "[|(h,l)::\<preceq>(G,lT); h\<le>|h'; G\<turnstile>h h'\<surd> |] ==> (h',l)::\<preceq>(G,lT)"
+apply( fast dest: conforms_localD elim!: conformsI lconf_hext)
+done
+
+lemma conforms_upd_obj: "[|(h,l)::\<preceq>(G, lT); G,h(a\<mapsto>obj)\<turnstile>obj\<surd>; h\<le>|h(a\<mapsto>obj)|] ==> (h(a\<mapsto>obj),l)::\<preceq>(G, lT)"
+apply( rule conforms_hext)
+apply   auto
+apply( rule hconfI)
+apply( drule conforms_heapD)
+apply( tactic {* auto_tac (HOL_cs addEs [thm "oconf_hext"] addDs [thm "hconfD"], simpset() delsimps [split_paired_All]) *})
+done
+
+lemma conforms_upd_local: 
+"[|(h, l)::\<preceq>(G, lT); G,h\<turnstile>v::\<preceq>T; lT va = Some T|] ==> (h, l(va\<mapsto>v))::\<preceq>(G, lT)"
+apply (unfold conforms_def)
+apply( auto elim: lconf_upd)
+done
 
 end
