src/HOL/MicroJava/J/Decl.thy
@@ -6,52 +6,58 @@
 Class declarations and programs
 *)
 
-Decl = Type +
+theory Decl = Type:
 
 types	fdecl		(* field declaration, cf. 8.3 (, 9.3) *)
-	= "vname \\<times> ty"
+	= "vname \<times> ty"
 
 
 types	sig		(* signature of a method, cf. 8.4.2 *)
-	= "mname \\<times> ty list"
+	= "mname \<times> ty list"
 
 	'c mdecl		(* method declaration in a class *)
-	= "sig \\<times> ty \\<times> 'c"
+	= "sig \<times> ty \<times> 'c"
 
 types	'c class		(* class *)
-	= "cname \\<times> fdecl list \\<times> 'c mdecl list"
+	= "cname \<times> fdecl list \<times> 'c mdecl list"
 	(* superclass, fields, methods*)
 
 	'c cdecl		(* class declaration, cf. 8.1 *)
-	= "cname \\<times> 'c class"
+	= "cname \<times> 'c class"
 
 consts
 
   Object  :: cname	(* name of root class *)
-  ObjectC :: 'c cdecl	(* decl of root class *)
+  ObjectC :: "'c cdecl"	(* decl of root class *)
 
 defs 
 
- ObjectC_def "ObjectC == (Object, (arbitrary, [], []))"
+ ObjectC_def: "ObjectC == (Object, (arbitrary, [], []))"
 
 
 types 'c prog = "'c cdecl list"
 
 
 translations
-  "fdecl"   <= (type) "vname \\<times> ty"
-  "sig"     <= (type) "mname \\<times> ty list"
-  "mdecl c" <= (type) "sig \\<times> ty \\<times> c"
-  "class c" <= (type) "cname \\<times> fdecl list \\<times> (c mdecl) list"
-  "cdecl c" <= (type) "cname \\<times> (c class)"
+  "fdecl"   <= (type) "vname \<times> ty"
+  "sig"     <= (type) "mname \<times> ty list"
+  "mdecl c" <= (type) "sig \<times> ty \<times> c"
+  "class c" <= (type) "cname \<times> fdecl list \<times> (c mdecl) list"
+  "cdecl c" <= (type) "cname \<times> (c class)"
   "prog  c" <= (type) "(c cdecl) list"
 
 constdefs
 
-  class		:: "'c prog => (cname \\<leadsto> 'c class)"
-  "class        \\<equiv> map_of"
+  class		:: "'c prog => (cname \<leadsto> 'c class)"
+  "class        \<equiv> map_of"
   is_class	:: "'c prog => cname => bool"
- "is_class G C  \\<equiv> class G C \\<noteq> None"
+ "is_class G C  \<equiv> class G C \<noteq> None"
+
+lemma finite_is_class: "finite {C. is_class G C}"
+apply (unfold is_class_def class_def)
+apply (fold dom_def)
+apply (rule finite_dom_map_of)
+done
 
 consts
 
