src/HOL/MicroJava/J/JBasis.thy
@@ -6,11 +6,69 @@
 Some auxiliary definitions.
 *)
 
-JBasis = Main + 
+theory JBasis = Main: 
 
+lemmas [simp] = Let_def
+
+section "unique"
+ 
 constdefs
 
   unique  :: "('a \\<times> 'b) list => bool"
  "unique  == nodups \\<circ> map fst"
 
+
+lemma fst_in_set_lemma [rule_format (no_asm)]: 
+      "(x, y) : set xys --> x : fst ` set xys"
+apply (induct_tac "xys")
+apply  auto
+done
+
+lemma unique_Nil [simp]: "unique []"
+apply (unfold unique_def)
+apply (simp (no_asm))
+done
+
+lemma unique_Cons [simp]: "unique ((x,y)#l) = (unique l & (!y. (x,y) ~: set l))"
+apply (unfold unique_def)
+apply (auto dest: fst_in_set_lemma)
+done
+
+lemma unique_append [rule_format (no_asm)]: "unique l' ==> unique l --> 
+ (!(x,y):set l. !(x',y'):set l'. x' ~= x) --> unique (l @ l')"
+apply (induct_tac "l")
+apply  (auto dest: fst_in_set_lemma)
+done
+
+lemma unique_map_inj [rule_format (no_asm)]: 
+  "unique l --> inj f --> unique (map (%(k,x). (f k, g k x)) l)"
+apply (induct_tac "l")
+apply  (auto dest: fst_in_set_lemma simp add: inj_eq)
+done
+
+section "More about Maps"
+
+lemma map_of_SomeI [rule_format (no_asm)]: 
+  "unique l --> (k, x) : set l --> map_of l k = Some x"
+apply (induct_tac "l")
+apply  auto
+done
+
+lemma Ball_set_table_: 
+  "(\\<forall>(x,y)\\<in>set l. P x y) --> (\\<forall>x. \\<forall>y. map_of l x = Some y --> P x y)"
+apply(induct_tac "l")
+apply(simp_all (no_asm))
+apply safe
+apply auto
+done
+lemmas Ball_set_table = Ball_set_table_ [THEN mp];
+
+lemma table_of_remap_SomeD [rule_format (no_asm)]: 
+"map_of (map (\<lambda>((k,k'),x). (k,(k',x))) t) k = Some (k',x) --> 
+ map_of t (k, k') = Some x"
+apply (induct_tac "t")
+apply  auto
+done
+
 end
+
