src/HOL/MicroJava/J/JTypeSafe.thy
@@ -3,7 +3,357 @@
     Author:     David von Oheimb
     Copyright   1999 Technische Universitaet Muenchen
 
-Type Safety of Java
+Type Safety Proof for MicroJava
 *)
 
-JTypeSafe = Eval + Conform
+theory JTypeSafe = Eval + Conform:
+
+declare split_beta [simp]
+
+lemma NewC_conforms: 
+"[|h a = None; (h, l)::\<preceq>(G, lT); wf_prog wf_mb G; is_class G C|] ==>  
+  (h(a\<mapsto>(C,(init_vars (fields (G,C))))), l)::\<preceq>(G, lT)"
+apply( erule conforms_upd_obj)
+apply(  unfold oconf_def)
+apply(  auto dest!: fields_is_type)
+done
+ 
+lemma Cast_conf: 
+ "[| wf_prog wf_mb G; G,h\<turnstile>v::\<preceq>Class C; G\<turnstile>C\<preceq>? D; cast_ok G D h v|]  
+  ==> G,h\<turnstile>v::\<preceq>Class D" 
+apply (unfold cast_ok_def)
+apply( case_tac "v = Null")
+apply(  simp)
+apply(  drule widen_RefT)
+apply(  clarify)
+apply( drule (1) non_npD)
+apply( auto intro!: conf_AddrI simp add: obj_ty_def)
+done
+
+lemma FAcc_type_sound: 
+"[| wf_prog wf_mb G; field (G,C) fn = Some (fd, ft); (h,l)::\<preceq>(G,lT);  
+  x' = None --> G,h\<turnstile>a'::\<preceq> Class C; np a' x' = None |] ==>  
+  G,h\<turnstile>the (snd (the (h (the_Addr a'))) (fn, fd))::\<preceq>ft"
+apply( drule np_NoneD)
+apply( erule conjE)
+apply( erule (1) notE impE)
+apply( drule non_np_objD)
+apply   auto
+apply( drule conforms_heapD [THEN hconfD])
+apply(  assumption)
+apply( drule (2) widen_cfs_fields)
+apply( drule (1) oconf_objD)
+apply auto
+done
+
+lemma FAss_type_sound: 
+ "[| wf_prog wf_mb G; a = the_Addr a'; (c, fs) = the (h a);  
+    (G, lT)\<turnstile>v::T'; G\<turnstile>T'\<preceq>ft;  
+    (G, lT)\<turnstile>aa::Class C;  
+    field (G,C) fn = Some (fd, ft); h''\<le>|h';  
+    x' = None --> G,h'\<turnstile>a'::\<preceq> Class C; h'\<le>|h;  
+    (h, l)::\<preceq>(G, lT); G,h\<turnstile>x::\<preceq>T'; np a' x' = None|] ==>  
+  h''\<le>|h(a\<mapsto>(c,(fs((fn,fd)\<mapsto>x)))) \<and>   
+  (h(a\<mapsto>(c,(fs((fn,fd)\<mapsto>x)))), l)::\<preceq>(G, lT) \<and>   
+  G,h(a\<mapsto>(c,(fs((fn,fd)\<mapsto>x))))\<turnstile>x::\<preceq>T'"
+apply( drule np_NoneD)
+apply( erule conjE)
+apply( simp)
+apply( drule non_np_objD)
+apply(   assumption)
+apply(  force)
+apply( clarify)
+apply( simp (no_asm_use))
+apply( frule (1) hext_objD)
+apply( erule exE)
+apply( simp)
+apply( clarify)
+apply( rule conjI)
+apply(  fast elim: hext_trans hext_upd_obj)
+apply( rule conjI)
+prefer 2
+apply(  fast elim: conf_upd_obj [THEN iffD2])
+
+apply( rule conforms_upd_obj)
+apply   auto
+apply(  rule_tac [2] hextI)
+prefer 2
+apply(  force)
+apply( rule oconf_hext)
+apply(  erule_tac [2] hext_upd_obj)
+apply( drule (2) widen_cfs_fields)
+apply( rule oconf_obj [THEN iffD2])
+apply( simp (no_asm))
+apply( intro strip)
+apply( case_tac "(aaa, b) = (fn, fd)")
+apply(  simp)
+apply(  fast intro: conf_widen)
+apply( fast dest: conforms_heapD [THEN hconfD] oconf_objD)
+done
+
+lemma Call_lemma2: "[| wf_prog wf_mb G; list_all2 (conf G h) pvs pTs;  
+   list_all2 (\<lambda>T T'. G\<turnstile>T\<preceq>T') pTs pTs'; wf_mhead G (mn,pTs') rT;  
+  length pTs' = length pns; nodups pns;  
+  Ball (set lvars) (split (\<lambda>vn. is_type G))  
+  |] ==> G,h\<turnstile>init_vars lvars(pns[\<mapsto>]pvs)[::\<preceq>]map_of lvars(pns[\<mapsto>]pTs')"
+apply (unfold wf_mhead_def)
+apply( clarsimp)
+apply( rule lconf_ext_list)
+apply(    rule Ball_set_table [THEN lconf_init_vars])
+apply(    force)
+apply(   assumption)
+apply(  assumption)
+apply( erule (2) conf_list_gext_widen)
+done
+
+lemma Call_type_sound: 
+ "[| wf_java_prog G; a' \<noteq> Null; (h, l)::\<preceq>(G, lT); class G C = Some y;  
+     max_spec G C (mn,pTsa) = {((mda,rTa),pTs')}; xc\<le>|xh; xh\<le>|h;  
+     list_all2 (conf G h) pvs pTsa; 
+     (md, rT, pns, lvars, blk, res) =  
+               the (method (G,fst (the (h (the_Addr a')))) (mn, pTs')); 
+  \<forall>lT. (h, init_vars lvars(pns[\<mapsto>]pvs)(This\<mapsto>a'))::\<preceq>(G, lT) -->  
+  (G, lT)\<turnstile>blk\<surd> -->  h\<le>|xi \<and>  (xi, xl)::\<preceq>(G, lT);  
+  \<forall>lT. (xi, xl)::\<preceq>(G, lT) --> (\<forall>T. (G, lT)\<turnstile>res::T -->  
+          xi\<le>|h' \<and> (h', xj)::\<preceq>(G, lT) \<and> (x' = None --> G,h'\<turnstile>v::\<preceq>T));  
+  G,xh\<turnstile>a'::\<preceq> Class C |] ==>  
+  xc\<le>|h' \<and> (h', l)::\<preceq>(G, lT) \<and>  (x' = None --> G,h'\<turnstile>v::\<preceq>rTa)"
+apply (unfold wf_java_prog_def)
+apply( drule max_spec2mheads)
+apply( clarify)
+apply( drule (2) non_np_objD')
+apply(  clarsimp)
+apply( clarsimp)
+apply( frule (1) hext_objD)
+apply( clarsimp)
+apply( drule (3) Call_lemma)
+apply( clarsimp simp add: wf_java_mdecl_def)
+apply( erule_tac V = "method ?sig ?x = ?y" in thin_rl)
+apply( drule spec, erule impE)
+apply(  erule_tac [2] notE impE, tactic "assume_tac 2")
+apply(  rule conformsI)
+apply(   erule conforms_heapD)
+apply(  rule lconf_ext)
+apply(   force elim!: Call_lemma2)
+apply(  erule conf_hext, erule (1) conf_obj_AddrI)
+apply( erule_tac V = "?E\<turnstile>?blk\<surd>" in thin_rl)
+apply( erule conjE)
+apply( drule spec, erule (1) impE)
+apply( drule spec, erule (1) impE)
+apply( erule_tac V = "?E\<turnstile>res::?rT" in thin_rl)
+apply( clarify)
+apply( rule conjI)
+apply(  fast intro: hext_trans)
+apply( rule conjI)
+apply(  rule_tac [2] impI)
+apply(  erule_tac [2] notE impE, tactic "assume_tac 2")
+apply(  frule_tac [2] conf_widen)
+apply(    tactic "assume_tac 4")
+apply(   tactic "assume_tac 2")
+prefer 2
+apply(  fast elim!: widen_trans)
+apply( erule conforms_hext)
+apply(  erule (1) hext_trans)
+apply( erule conforms_heapD)
+done
+
+declare split_if [split del]
+declare fun_upd_apply [simp del]
+declare fun_upd_same [simp]
+ML{*
+val forward_hyp_tac = ALLGOALS (TRY o (EVERY' [dtac spec, mp_tac,
+	(mp_tac ORELSE' (dtac spec THEN' mp_tac)), REPEAT o (etac conjE)]))
+*}
+ML{*
+Unify.search_bound := 40;
+Unify.trace_bound  := 40
+*}
+theorem eval_evals_exec_type_sound: 
+"wf_java_prog G ==>  
+  (G\<turnstile>(x,(h,l)) -e  \<succ>v  -> (x', (h',l')) -->  
+      (\<forall>lT.   (h ,l )::\<preceq>(G,lT) --> (\<forall>T . (G,lT)\<turnstile>e  :: T -->  
+      h\<le>|h' \<and> (h',l')::\<preceq>(G,lT) \<and> (x'=None --> G,h'\<turnstile>v  ::\<preceq> T )))) \<and>  
+  (G\<turnstile>(x,(h,l)) -es[\<succ>]vs-> (x', (h',l')) -->  
+      (\<forall>lT.   (h ,l )::\<preceq>(G,lT) --> (\<forall>Ts. (G,lT)\<turnstile>es[::]Ts -->  
+      h\<le>|h' \<and> (h',l')::\<preceq>(G,lT) \<and> (x'=None --> list_all2 (\<lambda>v T. G,h'\<turnstile>v::\<preceq>T) vs Ts)))) \<and>  
+  (G\<turnstile>(x,(h,l)) -c       -> (x', (h',l')) -->  
+      (\<forall>lT.   (h ,l )::\<preceq>(G,lT) -->       (G,lT)\<turnstile>c  \<surd> -->  
+      h\<le>|h' \<and> (h',l')::\<preceq>(G,lT)))"
+apply( rule eval_evals_exec_induct)
+apply( unfold c_hupd_def)
+
+(* several simplifications, XcptE, XcptEs, XcptS, Skip, Nil?? *)
+apply( simp_all)
+apply( tactic "ALLGOALS strip_tac")
+apply( tactic {* ALLGOALS (eresolve_tac (thms "ty_expr_ty_exprs_wt_stmt.elims") THEN_ALL_NEW Full_simp_tac) *})
+apply( tactic "ALLGOALS (EVERY' [REPEAT o (etac conjE), REPEAT o hyp_subst_tac])")
+apply( unfold wf_java_prog_def)
+
+(* Level 7 *)
+
+(* 15 NewC *)
+apply( drule new_AddrD)
+apply( erule disjE)
+prefer 2
+apply(  simp (no_asm_simp))
+apply( clarsimp)
+apply( rule conjI)
+apply(  force elim!: NewC_conforms)
+apply( rule conf_obj_AddrI)
+apply(  rule_tac [2] rtrancl_refl)
+apply( simp (no_asm))
+
+(* for Cast *)
+defer 1
+
+(* 14 Lit *)
+apply( erule conf_litval)
+
+(* 13 BinOp *)
+apply (tactic "forward_hyp_tac")
+apply (tactic "forward_hyp_tac")
+apply( rule conjI, erule (1) hext_trans)
+apply( erule conjI)
+apply( clarsimp)
+apply( drule eval_no_xcpt)
+apply( simp split add: binop.split)
+
+(* 12 LAcc *)
+apply( fast elim: conforms_localD [THEN lconfD])
+
+(* for FAss *)
+apply( tactic {* EVERY'[eresolve_tac (thms "ty_expr_ty_exprs_wt_stmt.elims") THEN_ALL_NEW Full_simp_tac, REPEAT o (etac conjE), hyp_subst_tac] 3*})
+
+(* for if *)
+apply( tactic {* (case_tac "the_Bool v" THEN_ALL_NEW Asm_full_simp_tac) 8*})
+
+apply (tactic "forward_hyp_tac")
+
+(* 11+1 if *)
+prefer 8
+apply(  fast intro: hext_trans)
+prefer 8
+apply(  fast intro: hext_trans)
+
+(* 10 Expr *)
+prefer 6
+apply( fast)
+
+(* 9 ??? *)
+apply( simp_all)
+
+(* 8 Cast *)
+prefer 8
+apply (rule impI)
+apply (drule raise_if_NoneD)
+apply (clarsimp)
+apply (fast elim: Cast_conf)
+
+(* 7 LAss *)
+apply (fold fun_upd_def)
+apply( tactic {* (eresolve_tac (thms "ty_expr_ty_exprs_wt_stmt.elims") THEN_ALL_NEW Full_simp_tac) 1 *})
+apply( blast intro: conforms_upd_local conf_widen)
+
+(* 6 FAcc *)
+apply( fast elim!: FAcc_type_sound)
+
+(* 5 While *)
+prefer 5
+apply(erule_tac V = "?a \<longrightarrow> ?b" in thin_rl)
+apply(drule (1) ty_expr_ty_exprs_wt_stmt.Loop)
+apply(force elim: hext_trans)
+
+apply (tactic "forward_hyp_tac")
+
+(* 4 Cons *)
+prefer 3
+apply( fast dest: evals_no_xcpt intro: conf_hext hext_trans)
+
+(* 3 ;; *)
+prefer 3
+apply( fast intro: hext_trans)
+
+(* 2 FAss *)
+apply( case_tac "x2 = None")
+prefer 2
+apply(  simp (no_asm_simp))
+apply(  fast intro: hext_trans)
+apply( simp)
+apply( drule eval_no_xcpt)
+apply( erule FAss_type_sound, simp (no_asm) (*###rule refl*), assumption+)
+
+apply( tactic prune_params_tac)
+(* Level 52 *)
+
+(* 1 Call *)
+apply( case_tac "x")
+prefer 2
+apply(  clarsimp)
+apply(  drule exec_xcpt)
+apply(  simp)
+apply(  drule_tac eval_xcpt)
+apply(  simp)
+apply(  fast elim: hext_trans)
+apply( clarify)
+apply( drule evals_no_xcpt)
+apply( simp)
+apply( case_tac "a' = Null")
+apply(  simp)
+apply(  drule exec_xcpt)
+apply(  simp)
+apply(  drule eval_xcpt)
+apply(  simp)
+apply(  fast elim: hext_trans)
+apply( drule (1) ty_expr_is_type)
+apply(clarsimp)
+apply(unfold is_class_def)
+apply(clarsimp)
+apply(rule Call_type_sound [unfolded wf_java_prog_def]);
+prefer 11
+apply blast
+apply (simp (no_asm_simp))+
+done
+ML{*
+Unify.search_bound := 20;
+Unify.trace_bound  := 20
+*}
+
+lemma eval_type_sound: "!!E s s'.  
+  [| G=prg E; wf_java_prog G; G\<turnstile>(x,s) -e\<succ>v -> (x',s'); s::\<preceq>E; E\<turnstile>e::T |]  
+  ==> s'::\<preceq>E \<and> (x'=None --> G,heap s'\<turnstile>v::\<preceq>T)"
+apply( simp (no_asm_simp) only: split_tupled_all)
+apply (drule eval_evals_exec_type_sound 
+             [THEN conjunct1, THEN mp, THEN spec, THEN mp])
+apply auto
+done
+
+lemma exec_type_sound: "!!E s s'.  
+  [| G=prg E; wf_java_prog G; G\<turnstile>(x,s) -s0-> (x',s'); s::\<preceq>E; E\<turnstile>s0\<surd> |]  
+  ==> s'::\<preceq>E"
+apply( simp (no_asm_simp) only: split_tupled_all)
+apply (drule eval_evals_exec_type_sound 
+             [THEN conjunct2, THEN conjunct2, THEN mp, THEN spec, THEN mp])
+apply   auto
+done
+
+theorem all_methods_understood: 
+"[|G=prg E; wf_java_prog G; G\<turnstile>(x,s) -e\<succ>a'-> Norm s'; a' \<noteq> Null; 
+          s::\<preceq>E; E\<turnstile>e::Class C; method (G,C) sig \<noteq> None|] ==>  
+  method (G,fst (the (heap s' (the_Addr a')))) sig \<noteq> None"
+apply( drule (4) eval_type_sound)
+apply(clarsimp)
+apply(unfold wf_java_prog_def)
+apply( frule widen_methd)
+apply(   assumption)
+prefer 2
+apply(  fast)
+apply( drule non_npD)
+apply auto
+done
+
+declare split_beta [simp del]
+declare fun_upd_apply [simp]
+
+end
+
+
