src/HOL/MicroJava/J/WellForm.thy
@@ -14,31 +14,410 @@ simplifications:
 * for uniformity, Object is assumed to be declared like any other class
 *)
 
-WellForm = TypeRel +
+theory WellForm = TypeRel:
 
-types 'c wf_mb = 'c prog => cname => 'c mdecl => bool
+types 'c wf_mb = "'c prog => cname => 'c mdecl => bool"
 
 constdefs
  wf_fdecl :: "'c prog => fdecl => bool"
-"wf_fdecl G == \\<lambda>(fn,ft). is_type G ft"
+"wf_fdecl G == \<lambda>(fn,ft). is_type G ft"
 
  wf_mhead :: "'c prog => sig => ty => bool"
-"wf_mhead G == \\<lambda>(mn,pTs) rT. (\\<forall>T\\<in>set pTs. is_type G T) \\<and> is_type G rT"
+"wf_mhead G == \<lambda>(mn,pTs) rT. (\<forall>T\<in>set pTs. is_type G T) \<and> is_type G rT"
 
  wf_mdecl :: "'c wf_mb => 'c wf_mb"
-"wf_mdecl wf_mb G C == \\<lambda>(sig,rT,mb). wf_mhead G sig rT \\<and> wf_mb G C (sig,rT,mb)"
+"wf_mdecl wf_mb G C == \<lambda>(sig,rT,mb). wf_mhead G sig rT \<and> wf_mb G C (sig,rT,mb)"
 
  wf_cdecl :: "'c wf_mb => 'c prog => 'c cdecl => bool"
 "wf_cdecl wf_mb G ==
-   \\<lambda>(C,(D,fs,ms)).
-  (\\<forall>f\\<in>set fs. wf_fdecl G         f) \\<and>  unique fs \\<and>
-  (\\<forall>m\\<in>set ms. wf_mdecl wf_mb G C m) \\<and>  unique ms \\<and>
-  (C \\<noteq> Object \\<longrightarrow> is_class G D \\<and>  \\<not>G\\<turnstile>D\\<preceq>C C \\<and>
-                   (\\<forall>(sig,rT,b)\\<in>set ms. \\<forall>D' rT' b'.
-                      method(G,D) sig = Some(D',rT',b') --> G\\<turnstile>rT\\<preceq>rT'))"
+   \<lambda>(C,(D,fs,ms)).
+  (\<forall>f\<in>set fs. wf_fdecl G         f) \<and>  unique fs \<and>
+  (\<forall>m\<in>set ms. wf_mdecl wf_mb G C m) \<and>  unique ms \<and>
+  (C \<noteq> Object \<longrightarrow> is_class G D \<and>  \<not>G\<turnstile>D\<preceq>C C \<and>
+                   (\<forall>(sig,rT,b)\<in>set ms. \<forall>D' rT' b'.
+                      method(G,D) sig = Some(D',rT',b') --> G\<turnstile>rT\<preceq>rT'))"
 
  wf_prog :: "'c wf_mb => 'c prog => bool"
 "wf_prog wf_mb G ==
-   let cs = set G in ObjectC \\<in> cs \\<and> (\\<forall>c\\<in>cs. wf_cdecl wf_mb G c) \\<and> unique G"
+   let cs = set G in ObjectC \<in> cs \<and> (\<forall>c\<in>cs. wf_cdecl wf_mb G c) \<and> unique G"
+
+lemma class_wf: 
+ "[|class G C = Some c; wf_prog wf_mb G|] ==> wf_cdecl wf_mb G (C,c)"
+apply (unfold wf_prog_def class_def)
+apply (simp)
+apply (fast dest: map_of_SomeD)
+done
+
+lemma class_Object [simp]: 
+	"wf_prog wf_mb G ==> class G Object = Some (arbitrary, [], [])"
+apply (unfold wf_prog_def ObjectC_def class_def)
+apply (auto intro: map_of_SomeI)
+done
+
+lemma is_class_Object [simp]: "wf_prog wf_mb G ==> is_class G Object"
+apply (unfold is_class_def)
+apply (simp (no_asm_simp))
+done
+
+lemma subcls1_wfD: "[|G\<turnstile>C\<prec>C1D; wf_prog wf_mb G|] ==> D \<noteq> C \<and> \<not>(D,C)\<in>(subcls1 G)^+"
+apply( frule r_into_trancl)
+apply( drule subcls1D)
+apply(clarify)
+apply( drule (1) class_wf)
+apply( unfold wf_cdecl_def)
+apply(force simp add: reflcl_trancl [THEN sym] simp del: reflcl_trancl)
+done
+
+lemma wf_cdecl_supD: 
+"!!r. \<lbrakk>wf_cdecl wf_mb G (C,D,r); C \<noteq> Object\<rbrakk> \<Longrightarrow> is_class G D"
+apply (unfold wf_cdecl_def)
+apply (auto split add: option.split_asm)
+done
+
+lemma subcls_asym: "[|wf_prog wf_mb G; (C,D)\<in>(subcls1 G)^+|] ==> \<not>(D,C)\<in>(subcls1 G)^+"
+apply(erule tranclE)
+apply(fast dest!: subcls1_wfD )
+apply(fast dest!: subcls1_wfD intro: trancl_trans)
+done
+
+lemma subcls_irrefl: "[|wf_prog wf_mb G; (C,D)\<in>(subcls1 G)^+|] ==> C \<noteq> D"
+apply (erule trancl_trans_induct)
+apply  (auto dest: subcls1_wfD subcls_asym)
+done
+
+lemma acyclic_subcls1: "wf_prog wf_mb G ==> acyclic (subcls1 G)"
+apply (unfold acyclic_def)
+apply (fast dest: subcls_irrefl)
+done
+
+lemma wf_subcls1: "wf_prog wf_mb G ==> wf ((subcls1 G)^-1)"
+apply (rule finite_acyclic_wf)
+apply ( subst finite_converse)
+apply ( rule finite_subcls1)
+apply (subst acyclic_converse)
+apply (erule acyclic_subcls1)
+done
+
+lemma subcls_induct: 
+"[|wf_prog wf_mb G; !!C. \<forall>D. (C,D)\<in>(subcls1 G)^+ --> P D ==> P C|] ==> P C"
+(is "?A \<Longrightarrow> PROP ?P \<Longrightarrow> _")
+proof -
+  assume p: "PROP ?P"
+  assume ?A thus ?thesis apply -
+apply(drule wf_subcls1)
+apply(drule wf_trancl)
+apply(simp only: trancl_converse)
+apply(erule_tac a = C in wf_induct)
+apply(rule p)
+apply(auto)
+done
+qed
+
+lemma subcls1_induct:
+"[|is_class G C; wf_prog wf_mb G; P Object;  
+   !!C D fs ms. [|C \<noteq> Object; is_class G C; class G C = Some (D,fs,ms) \<and>  
+    wf_cdecl wf_mb G (C,D,fs,ms) \<and> G\<turnstile>C\<prec>C1D \<and> is_class G D \<and> P D|] ==> P C 
+ |] ==> P C"
+(is "?A \<Longrightarrow> ?B \<Longrightarrow> ?C \<Longrightarrow> PROP ?P \<Longrightarrow> _")
+proof -
+  assume p: "PROP ?P"
+  assume ?A ?B ?C thus ?thesis apply -
+apply(unfold is_class_def)
+apply( rule impE)
+prefer 2
+apply(   assumption)
+prefer 2
+apply(  assumption)
+apply( erule thin_rl)
+apply( rule subcls_induct)
+apply(  assumption)
+apply( rule impI)
+apply( case_tac "C = Object")
+apply(  fast)
+apply safe
+apply( frule (1) class_wf)
+apply( frule (1) wf_cdecl_supD)
+
+apply( subgoal_tac "G\<turnstile>C\<prec>C1a")
+apply( erule_tac [2] subcls1I)
+apply(  rule p)
+apply (unfold is_class_def)
+apply auto
+done
+qed
+
+lemmas method_rec = wf_subcls1 [THEN [2] method_rec_lemma];
+
+lemmas fields_rec = wf_subcls1 [THEN [2] fields_rec_lemma];
+
+lemma method_Object [simp]: "wf_prog wf_mb G ==> method (G,Object) = empty"
+apply(subst method_rec)
+apply auto
+done
+
+lemma fields_Object [simp]: "wf_prog wf_mb G ==> fields (G,Object) = []"
+apply(subst fields_rec)
+apply auto
+done
+
+lemma field_Object [simp]: "wf_prog wf_mb G ==> field (G,Object) = empty"
+apply (unfold field_def)
+apply(simp (no_asm_simp))
+done
+
+lemma subcls_C_Object: "[|is_class G C; wf_prog wf_mb G|] ==> G\<turnstile>C\<preceq>C Object"
+apply(erule subcls1_induct)
+apply(  assumption)
+apply( fast)
+apply(auto dest!: wf_cdecl_supD)
+apply(erule (1) rtrancl_into_rtrancl2)
+done
+
+lemma is_type_rTI: "wf_mhead G sig rT ==> is_type G rT"
+apply (unfold wf_mhead_def)
+apply auto
+done
+
+lemma widen_fields_defpl': "[|is_class G C; wf_prog wf_mb G|] ==>  
+  \<forall>((fn,fd),fT)\<in>set (fields (G,C)). G\<turnstile>C\<preceq>C fd"
+apply( erule subcls1_induct)
+apply(   assumption)
+apply(  simp (no_asm_simp))
+apply( tactic "safe_tac HOL_cs")
+apply( subst fields_rec)
+apply(   assumption)
+apply(  assumption)
+apply( simp (no_asm) split del: split_if)
+apply( rule ballI)
+apply( simp (no_asm_simp) only: split_tupled_all)
+apply( simp (no_asm))
+apply( erule UnE)
+apply(  force)
+apply( erule r_into_rtrancl [THEN rtrancl_trans])
+apply auto
+done
+
+lemma widen_fields_defpl: "[|((fn,fd),fT) \<in> set (fields (G,C)); wf_prog wf_mb G; is_class G C|] ==>  
+  G\<turnstile>C\<preceq>C fd"
+apply( drule (1) widen_fields_defpl')
+apply (fast)
+done
+
+lemma unique_fields: "[|is_class G C; wf_prog wf_mb G|] ==> unique (fields (G,C))"
+apply( erule subcls1_induct)
+apply(   assumption)
+apply(  safe dest!: wf_cdecl_supD)
+apply(  simp (no_asm_simp))
+apply( drule subcls1_wfD)
+apply(  assumption)
+apply( subst fields_rec)
+apply   auto
+apply( rotate_tac -1)
+apply( frule class_wf)
+apply  auto
+apply( simp add: wf_cdecl_def)
+apply( erule unique_append)
+apply(  rule unique_map_inj)
+apply(   clarsimp)
+apply  (rule injI)
+apply(  simp)
+apply(auto dest!: widen_fields_defpl)
+done
+
+lemma fields_mono_lemma [rule_format (no_asm)]: "[|wf_prog wf_mb G; (C',C)\<in>(subcls1 G)^*|] ==>  
+  x \<in> set (fields (G,C)) --> x \<in> set (fields (G,C'))"
+apply(erule converse_rtrancl_induct)
+apply( safe dest!: subcls1D)
+apply(subst fields_rec)
+apply(  auto)
+done
+
+lemma fields_mono: 
+"\<lbrakk>map_of (fields (G,C)) fn = Some f; G\<turnstile>D\<preceq>C C; is_class G D; wf_prog wf_mb G\<rbrakk> 
+  \<Longrightarrow> map_of (fields (G,D)) fn = Some f"
+apply (rule map_of_SomeI)
+apply  (erule (1) unique_fields)
+apply (erule (1) fields_mono_lemma)
+apply (erule map_of_SomeD)
+done
+
+lemma widen_cfs_fields: 
+"[|field (G,C) fn = Some (fd, fT); G\<turnstile>D\<preceq>C C; wf_prog wf_mb G|]==>  
+  map_of (fields (G,D)) (fn, fd) = Some fT"
+apply (drule field_fields)
+apply (drule rtranclD)
+apply safe
+apply (frule subcls_is_class)
+apply (drule trancl_into_rtrancl)
+apply (fast dest: fields_mono)
+done
+
+lemma method_wf_mdecl [rule_format (no_asm)]: "wf_prog wf_mb G ==> is_class G C \<Longrightarrow>   
+     method (G,C) sig = Some (md,mh,m) 
+   --> G\<turnstile>C\<preceq>C md \<and> wf_mdecl wf_mb G md (sig,(mh,m))"
+apply( erule subcls1_induct)
+apply(   assumption)
+apply(  force)
+apply( clarify)
+apply( frule_tac C = C in method_rec)
+apply(  assumption)
+apply( rotate_tac -1)
+apply( simp)
+apply( drule override_SomeD)
+apply( erule disjE)
+apply(  erule_tac V = "?P --> ?Q" in thin_rl)
+apply (frule map_of_SomeD)
+apply (clarsimp simp add: wf_cdecl_def)
+apply( clarify)
+apply( rule rtrancl_trans)
+prefer 2
+apply(  assumption)
+apply( rule r_into_rtrancl)
+apply( fast intro: subcls1I)
+done
+
+lemma subcls_widen_methd [rule_format (no_asm)]: 
+  "[|G\<turnstile>T\<preceq>C T'; wf_prog wf_mb G|] ==>  
+   \<forall>D rT b. method (G,T') sig = Some (D,rT ,b) --> 
+  (\<exists>D' rT' b'. method (G,T) sig = Some (D',rT',b') \<and> G\<turnstile>rT'\<preceq>rT)"
+apply( drule rtranclD)
+apply( erule disjE)
+apply(  fast)
+apply( erule conjE)
+apply( erule trancl_trans_induct)
+prefer 2
+apply(  clarify)
+apply(  drule spec, drule spec, drule spec, erule (1) impE)
+apply(  fast elim: widen_trans)
+apply( clarify)
+apply( drule subcls1D)
+apply( clarify)
+apply( subst method_rec)
+apply(  assumption)
+apply( unfold override_def)
+apply( simp (no_asm_simp) del: split_paired_Ex)
+apply( case_tac "\<exists>z. map_of(map (\<lambda>(s,m). (s, ?C, m)) ms) sig = Some z")
+apply(  erule exE)
+apply(  rotate_tac -1, frule ssubst, erule_tac [2] asm_rl)
+prefer 2
+apply(  rotate_tac -1, frule ssubst, erule_tac [2] asm_rl)
+apply(  tactic "asm_full_simp_tac (HOL_ss addsimps [not_None_eq RS sym]) 1")
+apply(  simp_all (no_asm_simp) del: split_paired_Ex)
+apply( drule (1) class_wf)
+apply( simp (no_asm_simp) only: split_tupled_all)
+apply( unfold wf_cdecl_def)
+apply( drule map_of_SomeD)
+apply auto
+done
+
+lemma subtype_widen_methd: 
+ "[| G\<turnstile> C\<preceq>C D; wf_prog wf_mb G;  
+     method (G,D) sig = Some (md, rT, b) |]  
+  ==> \<exists>mD' rT' b'. method (G,C) sig= Some(mD',rT',b') \<and> G\<turnstile>rT'\<preceq>rT"
+apply(auto dest: subcls_widen_methd method_wf_mdecl simp add: wf_mdecl_def wf_mhead_def split_def)
+done
+
+lemma method_in_md [rule_format (no_asm)]: "wf_prog wf_mb G ==> is_class G C \<Longrightarrow> \<forall>D. method (G,C) sig = Some(D,mh,code) --> is_class G D \<and> method (G,D) sig = Some(D,mh,code)"
+apply (erule (1) subcls1_induct)
+ apply (simp)
+apply (erule conjE)
+apply (subst method_rec)
+  apply (assumption)
+ apply (assumption)
+apply (clarify)
+apply (erule_tac "x" = "Da" in allE)
+apply (clarsimp)
+ apply (simp add: map_of_map)
+ apply (clarify)
+ apply (subst method_rec)
+   apply (assumption)
+  apply (assumption)
+ apply (simp add: override_def map_of_map split add: option.split)
+done
+
+lemma widen_methd: 
+"[| method (G,C) sig = Some (md,rT,b); wf_prog wf_mb G; G\<turnstile>T''\<preceq>C C|] 
+  ==> \<exists>md' rT' b'. method (G,T'') sig = Some (md',rT',b') \<and> G\<turnstile>rT'\<preceq>rT"
+apply( drule subcls_widen_methd)
+apply   auto
+done
+
+lemma Call_lemma: 
+"[|method (G,C) sig = Some (md,rT,b); G\<turnstile>T''\<preceq>C C; wf_prog wf_mb G;  
+  class G C = Some y|] ==> \<exists>T' rT' b. method (G,T'') sig = Some (T',rT',b) \<and>  
+  G\<turnstile>rT'\<preceq>rT \<and> G\<turnstile>T''\<preceq>C T' \<and> wf_mhead G sig rT' \<and> wf_mb G T' (sig,rT',b)"
+apply( drule (2) widen_methd)
+apply( clarify)
+apply( frule subcls_is_class2)
+apply (unfold is_class_def)
+apply (simp (no_asm_simp))
+apply( drule method_wf_mdecl)
+apply( unfold wf_mdecl_def)
+apply( unfold is_class_def)
+apply auto
+done
+
+
+lemma fields_is_type_lemma [rule_format (no_asm)]: "[|is_class G C; wf_prog wf_mb G|] ==>  
+  \<forall>f\<in>set (fields (G,C)). is_type G (snd f)"
+apply( erule (1) subcls1_induct)
+apply(  simp (no_asm_simp))
+apply( subst fields_rec)
+apply(   fast)
+apply(  assumption)
+apply( clarsimp)
+apply( safe)
+prefer 2
+apply(  force)
+apply( drule (1) class_wf)
+apply( unfold wf_cdecl_def)
+apply( clarsimp)
+apply( drule (1) bspec)
+apply( unfold wf_fdecl_def)
+apply auto
+done
+
+lemma fields_is_type: "[|map_of (fields (G,C)) fn = Some f; wf_prog wf_mb G; is_class G C|] ==>  
+  is_type G f"
+apply(drule map_of_SomeD)
+apply(drule (2) fields_is_type_lemma)
+apply(auto)
+done
+
+lemma methd:
+  "[| wf_prog wf_mb G; (C,S,fs,mdecls) \<in> set G; (sig,rT,code) \<in> set mdecls |]
+  ==> method (G,C) sig = Some(C,rT,code) \<and> is_class G C"
+proof -
+  assume wf: "wf_prog wf_mb G" 
+  assume C:  "(C,S,fs,mdecls) \<in> set G"
+
+  assume m: "(sig,rT,code) \<in> set mdecls"
+  moreover
+  from wf
+  have "class G Object = Some (arbitrary, [], [])"
+    by simp 
+  moreover
+  from wf C
+  have c: "class G C = Some (S,fs,mdecls)"
+    by (auto simp add: wf_prog_def class_def is_class_def intro: map_of_SomeI)
+  ultimately
+  have O: "C \<noteq> Object"
+    by auto
+      
+  from wf C
+  have "unique mdecls"
+    by (unfold wf_prog_def wf_cdecl_def) auto
+
+  hence "unique (map (\<lambda>(s,m). (s,C,m)) mdecls)"
+    by - (induct mdecls, auto)
+
+  with m
+  have "map_of (map (\<lambda>(s,m). (s,C,m)) mdecls) sig = Some (C,rT,code)"
+    by (force intro: map_of_SomeI)
+
+  with wf C m c O
+  show ?thesis
+    by (auto simp add: is_class_def dest: method_rec)
+qed
 
 end
